@prefix : <http://www.semanticweb.org/defaultuser/ontologies/2020/7/Onto-CMDB#> .
@prefix owl: <http://www.w3.org/2002/07/owl#> .
@prefix rdf: <http://www.w3.org/1999/02/22-rdf-syntax-ns#> .
@prefix xml: <http://www.w3.org/XML/1998/namespace> .
@prefix xsd: <http://www.w3.org/2001/XMLSchema#> .
@prefix rdfs: <http://www.w3.org/2000/01/rdf-schema#> .
@prefix opla-sd: <http://ontologydesignpatterns.org/opla-sd#> .
@prefix ontodebug: <http://ainf.aau.at/ontodebug#> .
@base <http://www.semanticweb.org/defaultuser/ontologies/2020/7/Onto-CMDB> .

<http://www.semanticweb.org/defaultuser/ontologies/2020/7/Onto-CMDB> rdf:type owl:Ontology ;
                                                                      ontodebug:testCase [ ontodebug:axiom "hasProduct Range ManagedElement"^^xsd:string ;
                                                                                           ontodebug:type "true"^^xsd:boolean
                                                                                         ] ,
                                                                                         [ ontodebug:axiom "hasProduct Range ManagedSystemElement"^^xsd:string ;
                                                                                           ontodebug:type "true"^^xsd:boolean
                                                                                         ] ,
                                                                                         [ ontodebug:axiom "hasProduct Range PhysicalElement"^^xsd:string ;
                                                                                           ontodebug:type "true"^^xsd:boolean
                                                                                         ] ,
                                                                                         [ ontodebug:axiom "hasProduct Range SPDX"^^xsd:string ;
                                                                                           ontodebug:type "true"^^xsd:boolean
                                                                                         ] ,
                                                                                         [ ontodebug:axiom "FRU DisjointWith ManagedSystemElement"^^xsd:string ;
                                                                                           ontodebug:type "true"^^xsd:boolean
                                                                                         ] ,
                                                                                         [ ontodebug:axiom "ManagedSystemElement DisjointWith Product"^^xsd:string ;
                                                                                           ontodebug:type "true"^^xsd:boolean
                                                                                         ] ,
                                                                                         [ ontodebug:axiom "hasLocation Range SoftwareIdentity"^^xsd:string ;
                                                                                           ontodebug:type "false"^^xsd:boolean
                                                                                         ] ,
                                                                                         [ ontodebug:axiom "hasName Domain ManagedElement"^^xsd:string ;
                                                                                           ontodebug:type "true"^^xsd:boolean
                                                                                         ] ,
                                                                                         [ ontodebug:axiom "WarrantyDuration Domain SoftwareIdentity"^^xsd:string ;
                                                                                           ontodebug:type "false"^^xsd:boolean
                                                                                         ] ,
                                                                                         [ ontodebug:axiom "Product DisjointWith SoftwareIdentity"^^xsd:string ;
                                                                                           ontodebug:type "true"^^xsd:boolean
                                                                                         ] ,
                                                                                         [ ontodebug:axiom "WarrantyDuration Domain SPDX"^^xsd:string ;
                                                                                           ontodebug:type "false"^^xsd:boolean
                                                                                         ] ,
                                                                                         [ ontodebug:axiom "hasProduct Range SoftwareIdentity"^^xsd:string ;
                                                                                           ontodebug:type "true"^^xsd:boolean
                                                                                         ] ,
                                                                                         [ ontodebug:axiom "hasProduct Range FRU"^^xsd:string ;
                                                                                           ontodebug:type "true"^^xsd:boolean
                                                                                         ] ,
                                                                                         [ ontodebug:axiom "hasFRU Range Product"^^xsd:string ;
                                                                                           ontodebug:type "false"^^xsd:boolean
                                                                                         ] ,
                                                                                         [ ontodebug:axiom "Manufacturer Domain SoftwareIdentity"^^xsd:string ;
                                                                                           ontodebug:type "false"^^xsd:boolean
                                                                                         ] ,
                                                                                         [ ontodebug:axiom "Location SubClassOf ManagedSystemElement"^^xsd:string ;
                                                                                           ontodebug:type "false"^^xsd:boolean
                                                                                         ] ,
                                                                                         [ ontodebug:axiom "Classifications SubClassOf Product"^^xsd:string ;
                                                                                           ontodebug:type "false"^^xsd:boolean
                                                                                         ] ,
                                                                                         [ ontodebug:axiom "Manufacturer Domain ManagedElement"^^xsd:string ;
                                                                                           ontodebug:type "true"^^xsd:boolean
                                                                                         ] ,
                                                                                         [ ontodebug:axiom "Unknown Type Classifications"^^xsd:string ;
                                                                                           ontodebug:type "true"^^xsd:boolean
                                                                                         ] ,
                                                                                         [ ontodebug:axiom "FRU and Product SubClassOf ManagedElement"^^xsd:string ;
                                                                                           ontodebug:type "true"^^xsd:boolean
                                                                                         ] ,
                                                                                         [ ontodebug:axiom "Classifications DisjointWith OperatingStatus"^^xsd:string ;
                                                                                           ontodebug:type "true"^^xsd:boolean
                                                                                         ] ,
                                                                                         [ ontodebug:axiom "SPDX SubClassOf ManagedSystemElement"^^xsd:string ;
                                                                                           ontodebug:type "true"^^xsd:boolean
                                                                                         ] ,
                                                                                         [ ontodebug:axiom "OperatingStatus DisjointWith SoftwareIdentity"^^xsd:string ;
                                                                                           ontodebug:type "true"^^xsd:boolean
                                                                                         ] ,
                                                                                         [ ontodebug:axiom "hasName Domain ManagedSystemElement"^^xsd:string ;
                                                                                           ontodebug:type "true"^^xsd:boolean
                                                                                         ] ,
                                                                                         [ ontodebug:axiom "FRU SubClassOf ManagedSystemElement"^^xsd:string ;
                                                                                           ontodebug:type "false"^^xsd:boolean
                                                                                         ] ,
                                                                                         [ ontodebug:axiom "SPDX EquivalentTo SWID"^^xsd:string ;
                                                                                           ontodebug:type "false"^^xsd:boolean
                                                                                         ] ,
                                                                                         [ ontodebug:axiom "FRU DisjointWith SPDX"^^xsd:string ;
                                                                                           ontodebug:type "true"^^xsd:boolean
                                                                                         ] ,
                                                                                         [ ontodebug:axiom "Location DisjointWith ManagedSystemElement"^^xsd:string ;
                                                                                           ontodebug:type "true"^^xsd:boolean
                                                                                         ] ,
                                                                                         [ ontodebug:axiom "OperatingStatus Domain PhysicalElement"^^xsd:string ;
                                                                                           ontodebug:type "true"^^xsd:boolean
                                                                                         ] ,
                                                                                         [ ontodebug:axiom "Product SubClassOf ManagedSystemElement"^^xsd:string ;
                                                                                           ontodebug:type "false"^^xsd:boolean
                                                                                         ] ,
                                                                                         [ ontodebug:axiom "Caption Domain Location"^^xsd:string ;
                                                                                           ontodebug:type "true"^^xsd:boolean
                                                                                         ] ,
                                                                                         [ ontodebug:axiom "hasFRU Range FRU"^^xsd:string ;
                                                                                           ontodebug:type "true"^^xsd:boolean
                                                                                         ] ,
                                                                                         [ ontodebug:axiom "Family Domain FRU"^^xsd:string ;
                                                                                           ontodebug:type "false"^^xsd:boolean
                                                                                         ] ,
                                                                                         [ ontodebug:axiom "hasFRU Domain Product"^^xsd:string ;
                                                                                           ontodebug:type "false"^^xsd:boolean
                                                                                         ] ,
                                                                                         [ ontodebug:axiom "Caption Domain FRU"^^xsd:string ;
                                                                                           ontodebug:type "true"^^xsd:boolean
                                                                                         ] .

#################################################################
#    Annotation properties
#################################################################

###  http://ainf.aau.at/ontodebug#axiom
ontodebug:axiom rdf:type owl:AnnotationProperty ;
                rdfs:subPropertyOf ontodebug:testCase .


###  http://ainf.aau.at/ontodebug#testCase
ontodebug:testCase rdf:type owl:AnnotationProperty .


###  http://ainf.aau.at/ontodebug#type
ontodebug:type rdf:type owl:AnnotationProperty ;
               rdfs:subPropertyOf ontodebug:testCase .


###  http://ontologydesignpatterns.org/opla-sd#entityPosition
opla-sd:entityPosition rdf:type owl:AnnotationProperty .


###  http://ontologydesignpatterns.org/opla-sd#entityPositionX
opla-sd:entityPositionX rdf:type owl:AnnotationProperty .


###  http://ontologydesignpatterns.org/opla-sd#entityPositionY
opla-sd:entityPositionY rdf:type owl:AnnotationProperty .


#################################################################
#    Object Properties
#################################################################

###  http://www.semanticweb.org/defaultuser/ontologies/2020/7/Onto-CMDB#hasFRU
:hasFRU rdf:type owl:ObjectProperty ;
        rdfs:subPropertyOf owl:topObjectProperty ;
        rdfs:domain :PhysicalElement ;
        rdfs:range :FRU .


###  http://www.semanticweb.org/defaultuser/ontologies/2020/7/Onto-CMDB#hasLocation
:hasLocation rdf:type owl:ObjectProperty ;
             rdfs:domain :PhysicalElement ;
             rdfs:range :Location .


#################################################################
#    Data properties
#################################################################

###  http://www.semanticweb.org/defaultuser/ontologies/2020/7/Onto-CMDB#Address
:Address rdf:type owl:DatatypeProperty ;
         rdfs:subPropertyOf owl:topDataProperty ;
         rdfs:domain :Location ;
         rdfs:range xsd:string ;
         rdfs:comment "Address is a free-form string indicating a street, building, or other type of address for the location of the PhysicalElement."^^xsd:string .


###  http://www.semanticweb.org/defaultuser/ontologies/2020/7/Onto-CMDB#Caption
:Caption rdf:type owl:DatatypeProperty ;
         rdfs:subPropertyOf owl:topDataProperty ;
         rdfs:domain :ManagedElement ;
         rdfs:range xsd:string ;
         rdfs:comment "The Caption property is a short textual description (one- line string) of the object."^^xsd:string .


###  http://www.semanticweb.org/defaultuser/ontologies/2020/7/Onto-CMDB#Description
:Description rdf:type owl:DatatypeProperty ;
             rdfs:subPropertyOf owl:topDataProperty ;
             rdfs:domain :ManagedElement ;
             rdfs:range xsd:string ;
             rdfs:comment "The Description property provides a textual description of the object."^^xsd:string .


###  http://www.semanticweb.org/defaultuser/ontologies/2020/7/Onto-CMDB#ElementName
:ElementName rdf:type owl:DatatypeProperty ;
             rdfs:subPropertyOf owl:topDataProperty ;
             rdfs:domain :ManagedElement ;
             rdfs:range xsd:string ;
             rdfs:comment "A user-friendly name for the object. This property allows each instance to define a user-friendly name in addition to its key properties, identity data, and description information. Note that the Name property of ManagedSystemElement is also defined as a user-friendly name."^^xsd:string .


###  http://www.semanticweb.org/defaultuser/ontologies/2020/7/Onto-CMDB#EntitlementRequiredIndicator
:EntitlementRequiredIndicator rdf:type owl:DatatypeProperty ;
                              rdfs:subPropertyOf owl:topDataProperty ;
                              rdfs:domain :SWID ;
                              rdfs:range xsd:boolean ;
                              rdfs:comment """Identifies whether this application needs to match up with an entitlement for a reconciliation to be considered successful. Specifies if an entitlement is required to reconcile this application. See ISO/IEC 19770-2:2009 for guidance.
Example data format:
XX = entitlement status (true = entitlement required; false = no entitlement required)"""^^xsd:string .


###  http://www.semanticweb.org/defaultuser/ontologies/2020/7/Onto-CMDB#ExtendedResourceType
:ExtendedResourceType rdf:type owl:DatatypeProperty ;
                      rdfs:subPropertyOf owl:topDataProperty ;
                      rdfs:domain :SoftwareIdentity ;
                      rdfs:range xsd:integer ;
                      rdfs:comment "The binary format type of the installation package of the software."^^xsd:string .


###  http://www.semanticweb.org/defaultuser/ontologies/2020/7/Onto-CMDB#FRUNumber
:FRUNumber rdf:type owl:DatatypeProperty ;
           rdfs:subPropertyOf owl:topDataProperty ;
           rdfs:domain :FRU ;
           rdfs:range xsd:string ;
           rdfs:comment "FRU ordering information."^^xsd:string .


###  http://www.semanticweb.org/defaultuser/ontologies/2020/7/Onto-CMDB#Family
:Family rdf:type owl:DatatypeProperty ;
        rdfs:subPropertyOf owl:topDataProperty ;
        rdfs:domain :Product ;
        rdfs:range xsd:string ;
        rdfs:comment "Family that the product belongs to. A family refers to a set of products that are similar but not identical from a hardware or software point of view. Typically, a family is composed of different products, which have different configurations and pricing points. Products in the same family often have similar branding and cosmetic features."^^xsd:string .


###  http://www.semanticweb.org/defaultuser/ontologies/2020/7/Onto-CMDB#FullName
:FullName rdf:type owl:DatatypeProperty ;
          rdfs:subPropertyOf owl:topDataProperty ;
          rdfs:domain :SPDX ;
          rdfs:range xsd:string ;
          rdfs:comment "For example: MIT License or Apache License 2.0"^^xsd:string .


###  http://www.semanticweb.org/defaultuser/ontologies/2020/7/Onto-CMDB#Generation
:Generation rdf:type owl:DatatypeProperty ;
            rdfs:subPropertyOf owl:topDataProperty ;
            rdfs:domain :ManagedElement ;
            rdfs:range xsd:string ;
            rdfs:comment "Generation is an optional, monotonically increasing property that may be used to identify a particular generation of the resource represented by this class."^^xsd:string .


###  http://www.semanticweb.org/defaultuser/ontologies/2020/7/Onto-CMDB#IdentifyingNumber
:IdentifyingNumber rdf:type owl:DatatypeProperty ;
                   rdfs:subPropertyOf owl:topDataProperty ;
                   rdfs:domain :FRU ;
                   rdfs:range rdf:PlainLiteral ;
                   rdfs:comment "FRU identification such as a serial number on software or a die number on a hardware chip."^^xsd:string .


###  http://www.semanticweb.org/defaultuser/ontologies/2020/7/Onto-CMDB#InstallDate
:InstallDate rdf:type owl:DatatypeProperty ;
             rdfs:subPropertyOf owl:topDataProperty ;
             rdfs:domain :ManagedSystemElement ;
             rdfs:range xsd:dateTime ;
             rdfs:comment "A datetime value that indicates when the object was installed. Lack of a value does not indicate that the object is not installed."^^xsd:string .


###  http://www.semanticweb.org/defaultuser/ontologies/2020/7/Onto-CMDB#LargeBuildNumber
:LargeBuildNumber rdf:type owl:DatatypeProperty ;
                  rdfs:subPropertyOf owl:topDataProperty ;
                  rdfs:domain :SoftwareIdentity ;
                  rdfs:range xsd:integer ;
                  rdfs:comment "The build number of the software"^^xsd:string .


###  http://www.semanticweb.org/defaultuser/ontologies/2020/7/Onto-CMDB#MajorVersion
:MajorVersion rdf:type owl:DatatypeProperty ;
              rdfs:subPropertyOf owl:topDataProperty ;
              rdfs:domain :SoftwareIdentity ;
              rdfs:range xsd:integer ;
              rdfs:comment "The major number component of the software's version information - for example, '12' from version 12.1(3)T. This property is defined as a numeric value to allow the determination of 'newer' vs. 'older' releases. A 'newer' major release is indicated by a larger numeric value."^^xsd:string .


###  http://www.semanticweb.org/defaultuser/ontologies/2020/7/Onto-CMDB#ManufactureDate
:ManufactureDate rdf:type owl:DatatypeProperty ;
                 rdfs:subPropertyOf owl:topDataProperty ;
                 rdfs:domain :PhysicalElement ;
                 rdfs:range xsd:dateTime ;
                 rdfs:comment "The date that this PhysicalElement was manufactured"^^xsd:string .


###  http://www.semanticweb.org/defaultuser/ontologies/2020/7/Onto-CMDB#Manufacturer
:Manufacturer rdf:type owl:DatatypeProperty ;
              rdfs:subPropertyOf owl:topDataProperty ;
              rdfs:domain :PhysicalElement ;
              rdfs:range xsd:string ;
              rdfs:comment "The name of the organization responsible for producing the PhysicalElement. This organization might be the entity from whom the Element is purchased, but this is not necessarily true. The latter information is contained in the Vendor property of Product."^^xsd:string .


###  http://www.semanticweb.org/defaultuser/ontologies/2020/7/Onto-CMDB#MinorVersion
:MinorVersion rdf:type owl:DatatypeProperty ;
              rdfs:subPropertyOf owl:topDataProperty ;
              rdfs:domain :SoftwareIdentity ;
              rdfs:range xsd:integer ;
              rdfs:comment "The minor number component of the software's version information - for example, '1' from version 12.1(3)T. This property is defined as a numeric value to allow the determination of 'newer' vs. 'older' releases. A 'newer' minor release is indicated by a larger numeric value."^^xsd:string .


###  http://www.semanticweb.org/defaultuser/ontologies/2020/7/Onto-CMDB#Model
:Model rdf:type owl:DatatypeProperty ;
       rdfs:subPropertyOf owl:topDataProperty ;
       rdfs:domain :PhysicalElement ;
       rdfs:range xsd:string ;
       rdfs:comment "The name by which the PhysicalElement is generally known"^^xsd:string .


###  http://www.semanticweb.org/defaultuser/ontologies/2020/7/Onto-CMDB#Name
:Name rdf:type owl:DatatypeProperty ;
      rdfs:subPropertyOf owl:topDataProperty ;
      rdfs:domain :ManagedElement ;
      rdfs:range xsd:Name ;
      rdfs:comment "The Name property defines the label by which the object is known."^^xsd:string .


###  http://www.semanticweb.org/defaultuser/ontologies/2020/7/Onto-CMDB#Notes
:Notes rdf:type owl:DatatypeProperty ;
       rdfs:subPropertyOf owl:topDataProperty ;
       rdfs:domain :SPDX ;
       rdfs:range xsd:string ;
       rdfs:comment "Additional information about the license."^^xsd:string .


###  http://www.semanticweb.org/defaultuser/ontologies/2020/7/Onto-CMDB#OtherIdentifyingInfo
:OtherIdentifyingInfo rdf:type owl:DatatypeProperty ;
                      rdfs:subPropertyOf owl:topDataProperty ;
                      rdfs:domain :PhysicalElement ;
                      rdfs:range xsd:string ;
                      rdfs:comment "OtherIdentifyingInfo captures data in addition to Tag information. This information could be used to identify a Physical Element. One example is bar code data associated with an Element that also has an asset tag."^^xsd:string .


###  http://www.semanticweb.org/defaultuser/ontologies/2020/7/Onto-CMDB#PartNumber
:PartNumber rdf:type owl:DatatypeProperty ;
            rdfs:subPropertyOf owl:topDataProperty ;
            rdfs:domain :PhysicalElement ;
            rdfs:range xsd:string ;
            rdfs:comment "The part number assigned by the organization that is responsible for producing or manufacturing the PhysicalElement."^^xsd:string .


###  http://www.semanticweb.org/defaultuser/ontologies/2020/7/Onto-CMDB#PhysicalPosition
:PhysicalPosition rdf:type owl:DatatypeProperty ;
                  rdfs:subPropertyOf owl:topDataProperty ;
                  rdfs:domain :Location ;
                  rdfs:range xsd:string ;
                  rdfs:comment "Position is a free-form string that indicates the placement of a PhysicalElement. It can specify slot information on a HostingBoard, mounting site in a Cabinet, or latitude and longitude information, for example, from a GPS. It is part of the key of the Location object."^^xsd:string .


###  http://www.semanticweb.org/defaultuser/ontologies/2020/7/Onto-CMDB#PrimaryStatus
:PrimaryStatus rdf:type owl:DatatypeProperty ;
               rdfs:subPropertyOf owl:topDataProperty ;
               rdfs:domain :ManagedSystemElement ;
               rdfs:range rdf:PlainLiteral .


###  http://www.semanticweb.org/defaultuser/ontologies/2020/7/Onto-CMDB#ProductTitle
:ProductTitle rdf:type owl:DatatypeProperty ;
              rdfs:subPropertyOf owl:topDataProperty ;
              rdfs:domain :SWID ;
              rdfs:range xsd:string ;
              rdfs:comment "Identifies the application. Accurately identifies the application. See ISO/IEC 19770-2:2009 for guidance."^^xsd:string .


###  http://www.semanticweb.org/defaultuser/ontologies/2020/7/Onto-CMDB#ProductVersion
:ProductVersion rdf:type owl:DatatypeProperty ;
                rdfs:subPropertyOf owl:topDataProperty ;
                rdfs:domain :SWID ;
                rdfs:range xsd:string ;
                rdfs:comment "Accurately identifies the application version. Identifies the application version using two values – numeric version and version string. See ISO/IEC 19770-2:2009 for guidance."^^xsd:string .


###  http://www.semanticweb.org/defaultuser/ontologies/2020/7/Onto-CMDB#ReleaseDate
:ReleaseDate rdf:type owl:DatatypeProperty ;
             rdfs:subPropertyOf owl:topDataProperty ;
             rdfs:domain :SoftwareIdentity ;
             rdfs:range xsd:dateTime ;
             rdfs:comment "The date the software was released."^^xsd:string .


###  http://www.semanticweb.org/defaultuser/ontologies/2020/7/Onto-CMDB#RevisionLevel
:RevisionLevel rdf:type owl:DatatypeProperty ;
               rdfs:subPropertyOf owl:topDataProperty ;
               rdfs:domain :FRU ;
               rdfs:range xsd:string ;
               rdfs:comment "The FRU's revision level."^^xsd:string .


###  http://www.semanticweb.org/defaultuser/ontologies/2020/7/Onto-CMDB#RevisionNumber
:RevisionNumber rdf:type owl:DatatypeProperty ;
                rdfs:subPropertyOf owl:topDataProperty ;
                rdfs:domain :SoftwareIdentity ;
                rdfs:range xsd:integer ;
                rdfs:comment "The revision or maintenance release component of the software's version information - for example, '3' from version 12.1(3)T. This property is defined as a numeric value to allow the determination of 'newer' vs. 'older' releases. A 'newer' revision is indicated by a larger numeric value."^^xsd:string .


###  http://www.semanticweb.org/defaultuser/ontologies/2020/7/Onto-CMDB#SKU
:SKU rdf:type owl:DatatypeProperty ;
     rdfs:subPropertyOf owl:topDataProperty ;
     rdfs:domain :Product ;
     rdfs:range xsd:string ;
     rdfs:comment "The stock-keeping unit number."^^xsd:string .


###  http://www.semanticweb.org/defaultuser/ontologies/2020/7/Onto-CMDB#SerialNumber
:SerialNumber rdf:type owl:DatatypeProperty ;
              rdfs:subPropertyOf owl:topDataProperty ;
              rdfs:domain :PhysicalElement ;
              rdfs:range xsd:string ;
              rdfs:comment "A manufacturer-allocated number used to identify the Physical Element."^^xsd:string .


###  http://www.semanticweb.org/defaultuser/ontologies/2020/7/Onto-CMDB#ShortIdentifier
:ShortIdentifier rdf:type owl:DatatypeProperty ;
                 rdfs:subPropertyOf owl:topDataProperty ;
                 rdfs:domain :SPDX ;
                 rdfs:range xsd:string ;
                 rdfs:comment "A license identifier is a human readable short text string that uniquely identifies a license. For example: MIT"^^xsd:string .


###  http://www.semanticweb.org/defaultuser/ontologies/2020/7/Onto-CMDB#SoftwareCreator
:SoftwareCreator rdf:type owl:DatatypeProperty ;
                 rdfs:subPropertyOf owl:topDataProperty ;
                 rdfs:domain :SWID ;
                 rdfs:range xsd:string ;
                 rdfs:comment "Identifies the creator of the software.Identifies the application creator.See ISO/IEC 19770-2:2009 for guidance."^^xsd:string .


###  http://www.semanticweb.org/defaultuser/ontologies/2020/7/Onto-CMDB#SoftwareId
:SoftwareId rdf:type owl:DatatypeProperty ;
            rdfs:subPropertyOf owl:topDataProperty ;
            rdfs:domain :SWID ;
            rdfs:range xsd:string ;
            rdfs:comment "Identifies the specific version of a specific application. Accurately identifies the application. See ISO/IEC 19770-2:2009 for guidance."^^xsd:string .


###  http://www.semanticweb.org/defaultuser/ontologies/2020/7/Onto-CMDB#SoftwareLicensor
:SoftwareLicensor rdf:type owl:DatatypeProperty ;
                  rdfs:subPropertyOf owl:topDataProperty ;
                  rdfs:domain :SWID ;
                  rdfs:range xsd:string ;
                  rdfs:comment "Identifies the licensor who owns the software copyright. See ISO/IEC 19770-2:2009 for guidance."^^xsd:string .


###  http://www.semanticweb.org/defaultuser/ontologies/2020/7/Onto-CMDB#Tag
:Tag rdf:type owl:DatatypeProperty ;
     rdfs:subPropertyOf owl:topDataProperty ;
     rdfs:domain :PhysicalElement ;
     rdfs:range rdf:PlainLiteral ;
     rdfs:comment "An arbitrary string that uniquely identifies the Physical Element and serves as the key of the Element. The Tag property can contain information such as asset tag or serial number data. The key for PhysicalElement is placed very high in the object hierarchy in order to independently identify the hardware or entity, regardless of physical placement in or on Cabinets, Adapters, and so on. For example, a hotswappable or removable component can be taken from its containing (scoping) package and be temporarily unused. The object still continues to exist and can even be inserted into a different scoping container. Therefore, the key for Physical Element is an arbitrary string and is defined independently of any placement or location-oriented hierarchy."^^xsd:string .


###  http://www.semanticweb.org/defaultuser/ontologies/2020/7/Onto-CMDB#TagCreator
:TagCreator rdf:type owl:DatatypeProperty ;
            rdfs:subPropertyOf owl:topDataProperty ;
            rdfs:domain :SWID ;
            rdfs:range xsd:string ;
            rdfs:comment """Identifies the tag creator.Identifies the tag creator. See ISO/IEC 19770-2:2009 for guidance.
Example data format:
“regid.2007-01.com.agnitioadvisors,BU-A”
where:
regid = registered id
2007-01 = the year and first month the domain was registered (yyyy-mm)
com = the upper level domain
AgnitioAdvisors = the domain name
BU-A = the sub-unit creating the SWID tag
xxx = the name of the business unit (BU) that created the SWID tag
Note that everything after the comma ‘,’ is optional and only required if a software title is specific to a particular business unite."""^^xsd:string .


###  http://www.semanticweb.org/defaultuser/ontologies/2020/7/Onto-CMDB#TargetOperatingSystems
:TargetOperatingSystems rdf:type owl:DatatypeProperty ;
                        rdfs:subPropertyOf owl:topDataProperty ;
                        rdfs:domain :SoftwareIdentity ;
                        rdfs:range xsd:string ;
                        rdfs:comment """Specifies the target operating systems of the software.

Unknown, Other, MACOS, ATTUNIX, DGUX, DECNT, Tru64 UNIX, OpenVMS, HPUX, AIX, MVS, OS400, OS/2, JavaVM, MSDOS, WIN3x, WIN95, WIN98, WINNT, WINCE, NCR3000, NetWare, OSF, DC/OS, Reliant UNIX, SCO UnixWare, SCO OpenServer, Sequent, IRIX, Solaris, SunOS, U6000, ASERIES, HP NonStop OS, HP NonStop OSS, BS2000, LINUX, Lynx, XENIX, VM, Interactive UNIX, BSDUNIX, FreeBSD, NetBSD, GNU Hurd, OS9, MACH Kernel, Inferno, QNX, EPOC, IxWorks, VxWorks, MiNT, BeOS, HP MPE, NextStep, PalmPilot, Rhapsody, Windows 2000, Dedicated, OS/390, VSE, TPF, Windows (R) Me, Caldera Open UNIX, OpenBSD, Not Applicable, Windows XP, z/OS, Microsoft Windows Server 2003, Microsoft Windows Server 2003 64-Bit, Windows XP 64-Bit, Windows XP Embedded, Windows Vista, Windows Vista 64-Bit, Windows Embedded for Point of Service, Microsoft Windows Server 2008, Microsoft Windows Server 2008 64-Bit, FreeBSD 64-Bit, RedHat Enterprise Linux, RedHat Enterprise Linux 64-Bit, Solaris 64-Bit, SUSE, SUSE 64-Bit, SLES, SLES 64-Bit, Novell OES, Novell Linux Desktop, Sun Java Desktop System, Mandriva, Mandriva 64-Bit, TurboLinux, TurboLinux 64-Bit, Ubuntu, Ubuntu 64-Bit, Debian, Debian 64-Bit, Linux 2.4.x, Linux 2.4.x 64-Bit, Linux 2.6.x, Linux 2.6.x 64-Bit, Linux 64-Bit, Other 64-Bit, Microsoft Windows Server 2008 R2, VMware ESXi, Microsoft Windows 7, CentOS 32-bit, CentOS 64-bit, Oracle Linux 32-bit, Oracle Linux 64-bit, eComStation 32-bitx, Microsoft Windows Server 2011, Microsoft Windows Server 2012, Microsoft Windows 8, Microsoft Windows 8 64-bit, Microsoft Windows Server 2012 R2, Microsoft Windows Server 2016, Microsoft Windows 8.1, Microsoft Windows 8.1 64-bit, Microsoft Windows 10, Microsoft Windows 10 64-bit"""^^xsd:string .


###  http://www.semanticweb.org/defaultuser/ontologies/2020/7/Onto-CMDB#Text
:Text rdf:type owl:DatatypeProperty ;
      rdfs:subPropertyOf owl:topDataProperty ;
      rdfs:domain :SPDX ;
      rdfs:range xsd:string ;
      rdfs:comment """For example: 

Copyright (c) <year> <copyright holders>

Permission is hereby granted, free of charge, to any person obtaining a copy of this software and associated documentation files (the \"Software\"), to deal in the Software without restriction, including without limitation the rights to use, copy, modify, merge, publish, distribute, sublicense, and/or sell copies of the Software, and to permit persons to whom the Software is furnished to do so, subject to the following conditions:

The above copyright notice and this permission notice (including the next paragraph) shall be included in all copies or substantial portions of the Software.

THE SOFTWARE IS PROVIDED \"AS IS\", WITHOUT WARRANTY OF ANY KIND, EXPRESS OR IMPLIED, INCLUDING BUT NOT LIMITED TO THE WARRANTIES OF MERCHANTABILITY, FITNESS FOR A PARTICULAR PURPOSE AND NONINFRINGEMENT. IN NO EVENT SHALL THE AUTHORS OR COPYRIGHT HOLDERS BE LIABLE FOR ANY CLAIM, DAMAGES OR OTHER LIABILITY, WHETHER IN AN ACTION OF CONTRACT, TORT OR OTHERWISE, ARISING FROM, OUT OF OR IN CONNECTION WITH THE SOFTWARE OR THE USE OR OTHER DEALINGS IN THE SOFTWARE."""^^xsd:string .


###  http://www.semanticweb.org/defaultuser/ontologies/2020/7/Onto-CMDB#UserTracking
:UserTracking rdf:type owl:DatatypeProperty ;
              rdfs:subPropertyOf owl:topDataProperty ;
              rdfs:domain :PhysicalElement ;
              rdfs:range xsd:string ;
              rdfs:comment "User-assigned and writeable asset-tracking identifier for the PhysicalElement."^^xsd:string .


###  http://www.semanticweb.org/defaultuser/ontologies/2020/7/Onto-CMDB#Vendor
:Vendor rdf:type owl:DatatypeProperty ;
        rdfs:subPropertyOf owl:topDataProperty ;
        rdfs:domain :FRU ;
        rdfs:range rdf:PlainLiteral ;
        rdfs:comment "The name of the FRU's supplier."^^xsd:string .


###  http://www.semanticweb.org/defaultuser/ontologies/2020/7/Onto-CMDB#VendorEquipmentType
:VendorEquipmentType rdf:type owl:DatatypeProperty ;
                     rdfs:subPropertyOf owl:topDataProperty ;
                     rdfs:domain :PhysicalElement ;
                     rdfs:range xsd:string ;
                     rdfs:comment "A vendor-specific hardware type for the PhysicalElement. It describes the specific equipment type for the element, as defined by the vendor or manufacturer."^^xsd:string .


###  http://www.semanticweb.org/defaultuser/ontologies/2020/7/Onto-CMDB#Version
:Version rdf:type owl:DatatypeProperty ;
         rdfs:subPropertyOf owl:topDataProperty ;
         rdfs:domain :PhysicalElement ;
         rdfs:range xsd:string ;
         rdfs:comment "A string that indicates the version of the PhysicalElement"^^xsd:string .


###  http://www.semanticweb.org/defaultuser/ontologies/2020/7/Onto-CMDB#VersionString
:VersionString rdf:type owl:DatatypeProperty ;
               rdfs:subPropertyOf owl:topDataProperty ;
               rdfs:domain :SoftwareIdentity ;
               rdfs:range xsd:string ;
               rdfs:comment "A string representing the complete software version information - for example, '12.1(3)T'. This string and the numeric major/minor/revision/build properties are complementary. Since vastly different representations and semantics exist for versions, it is not assumed that one representation is sufficient to permit a client to perform computations (i.e., the values are numeric) and a user to recognize the software's version (i.e., the values are understandable and readable). Hence, both numeric and string representations of version are provided."^^xsd:string .


###  http://www.semanticweb.org/defaultuser/ontologies/2020/7/Onto-CMDB#WarrantyDuration
:WarrantyDuration rdf:type owl:DatatypeProperty ;
                  rdfs:subPropertyOf owl:topDataProperty ;
                  rdfs:domain :Product ;
                  rdfs:range xsd:integer ;
                  rdfs:comment "If this Product is under warranty, the duration of the warranty in days."^^xsd:string .


###  http://www.semanticweb.org/defaultuser/ontologies/2020/7/Onto-CMDB#WarrantyStartDate
:WarrantyStartDate rdf:type owl:DatatypeProperty ;
                   rdfs:subPropertyOf owl:topDataProperty ;
                   rdfs:domain :Product ;
                   rdfs:range xsd:string ;
                   rdfs:comment "If this Product is under warranty, the start date of the warranty."^^xsd:string .


###  http://www.semanticweb.org/defaultuser/ontologies/2020/7/Onto-CMDB#WebPages
:WebPages rdf:type owl:DatatypeProperty ;
          rdfs:subPropertyOf owl:topDataProperty ;
          rdfs:domain :SPDX ;
          rdfs:range xsd:string ;
          rdfs:comment "Other web pages for this license."^^xsd:string .


#################################################################
#    Classes
#################################################################

###  http://www.semanticweb.org/defaultuser/ontologies/2020/7/Onto-CMDB#Classifications
:Classifications rdf:type owl:Class ;
                 rdfs:subClassOf :SoftwareIdentity ;
                 rdfs:comment "Classify the software."^^xsd:string .


###  http://www.semanticweb.org/defaultuser/ontologies/2020/7/Onto-CMDB#FRU
:FRU rdf:type owl:Class ;
     rdfs:subClassOf :ManagedElement ;
     opla-sd:entityPosition [ opla-sd:entityPositionX "125.91659479562537"^^xsd:double ;
                              opla-sd:entityPositionY "45.88204538672695"^^xsd:double ;
                              rdfs:comment "This is an entity positioning annotation generated by CoModIDE (https://comodide.com/). Removing this annotation will break rendering the CoModIDE schema diagram view."@en
                            ] ;
     rdfs:comment "The FRU class is a vendor-defined collection of Products and/or PhysicalElements that is associated with a Product for the purpose of supporting, maintaining or upgrading that Product at the customer's location. FRU is an acronym for 'field replaceable unit'."^^xsd:string .


###  http://www.semanticweb.org/defaultuser/ontologies/2020/7/Onto-CMDB#HealthState
:HealthState rdf:type owl:Class ;
             rdfs:subClassOf :ManagedSystemElement ;
             rdfs:comment """Indicates the current health of the element. This attribute expresses the health of this element but not necessarily that of its subcomponents. 
\"Non-recoverable Error\" - The element has completely failed, and recovery is not possible. All functionality provided by this element has been lost. 
\"Critical Failure\"  - The element is non-functional and recovery might not be possible. 
\"Major Failure\" - The element is failing. It is possible that some or all of the functionality of this component is degraded or not working. 
\"Minor Failure\"  - All functionality is available but some might be degraded. 
\"Degraded/Warning\"  - The element is in working order and all functionality is provided. However, the element is not working to the best of its abilities. For example, the element might not be operating at optimal performance or it might be reporting recoverable errors. 
\"OK\"  - The element is fully functional and is operating within normal operational parameters and without error. \"Unknown\".

Values: Unknown, OK, Degraded/Warning, Minor failure, Major failure, Critical failure, Non-recoverable error"""^^xsd:string .


###  http://www.semanticweb.org/defaultuser/ontologies/2020/7/Onto-CMDB#Location
:Location rdf:type owl:Class ;
          rdfs:subClassOf :ManagedElement ;
          opla-sd:entityPosition [ opla-sd:entityPositionX "215.7828295953237"^^xsd:double ;
                                   opla-sd:entityPositionY "76.50558656596547"^^xsd:double ;
                                   rdfs:comment "This is an entity positioning annotation generated by CoModIDE (https://comodide.com/). Removing this annotation will break rendering the CoModIDE schema diagram view."@en
                                 ] ;
          rdfs:comment "The Location class specifies the position and address of a PhysicalElement."^^xsd:string .


###  http://www.semanticweb.org/defaultuser/ontologies/2020/7/Onto-CMDB#ManagedElement
:ManagedElement rdf:type owl:Class ;
                opla-sd:entityPosition [ opla-sd:entityPositionX "185.9162982628709"^^xsd:double ;
                                         opla-sd:entityPositionY "295.0637332535682"^^xsd:double ;
                                         rdfs:comment "This is an entity positioning annotation generated by CoModIDE (https://comodide.com/). Removing this annotation will break rendering the CoModIDE schema diagram view."@en
                                       ] ;
                rdfs:comment "ManagedElement is an abstract class that provides a common superclass."^^xsd:string .


###  http://www.semanticweb.org/defaultuser/ontologies/2020/7/Onto-CMDB#ManagedSystemElement
:ManagedSystemElement rdf:type owl:Class ;
                      rdfs:subClassOf :ManagedElement ;
                      opla-sd:entityPosition [ opla-sd:entityPositionX "360.1391270866579"^^xsd:double ;
                                               opla-sd:entityPositionY "400.1452533215478"^^xsd:double ;
                                               rdfs:comment "This is an entity positioning annotation generated by CoModIDE (https://comodide.com/). Removing this annotation will break rendering the CoModIDE schema diagram view."@en
                                             ] ;
                      rdfs:comment "Any distinguishable component of a System is a candidate for inclusion in this class. Examples of system components include: - software components such as application servers, databases, and applications - operating system components such as files, processes, and threads - device components such as disk drives, controllers, processors, and printers - physical components such as chips and cards."^^xsd:string .


###  http://www.semanticweb.org/defaultuser/ontologies/2020/7/Onto-CMDB#OperatingStatus
:OperatingStatus rdf:type owl:Class ;
                 rdfs:subClassOf :ManagedSystemElement ;
                 rdfs:comment """OperatingStatus provides a current status value for the operational condition of the element. It can also provide the transitional states when an element is transitioning from one state to another. 

\"Unknown\" indicates the implementation is in general capable of returning this property, but is unable to do so at this time. 
\"None\" indicates that the implementation (provider) is capable of returning a value for this property, but not ever for this particular piece of hardware/software or the property is intentionally not used because it adds no meaningful information (as in the case of a property that is intended to add additional info to another property). 
\"Servicing\" describes an element being configured, maintained, cleaned, or otherwise administered. 
\"Dormant\" indicates that the element is inactive or quiesced.
\"Migrating\" element is being moved between host elements. 
\"In Test\" element is performing test functions. 
\"Transitioning\" describes an element that is between states, that is, it is not fully available in either its previous state or its next state. This value should be used if other values indicating a transition to a specific state are not applicable. 
\"In Service\" describes an element that is in service and operational."""^^xsd:string .


###  http://www.semanticweb.org/defaultuser/ontologies/2020/7/Onto-CMDB#PhysicalElement
:PhysicalElement rdf:type owl:Class ;
                 rdfs:subClassOf :ManagedSystemElement ;
                 owl:disjointWith :SoftwareIdentity ;
                 opla-sd:entityPosition [ opla-sd:entityPositionX "509.96779175836207"^^xsd:double ;
                                          opla-sd:entityPositionY "129.97908426746073"^^xsd:double ;
                                          rdfs:comment "This is an entity positioning annotation generated by CoModIDE (https://comodide.com/). Removing this annotation will break rendering the CoModIDE schema diagram view."@en
                                        ] ;
                 rdfs:comment "Instances of this class can be defined as an object that can be seen or touched. All Processes, Files, and LogicalDevices are considered not to be Physical Elements. For example, it is not possible to touch the functionality of a 'modem.' You can touch only the card or package that implements the modem. The same card could also implement a LAN adapter. PhysicalElements are tangible ManagedSystemElements that have a physical manifestation of some sort. Note that the properties of PhysicalElement describe a hardware entity. Possible replacement (FRU) information is defined by FRU association. This definition allows a client to determine what hardware can be replaced (FRUed) and what 'spare' parts might be required by a customer or engineer doing the replacement."^^xsd:string .


###  http://www.semanticweb.org/defaultuser/ontologies/2020/7/Onto-CMDB#PrimaryStatus
:PrimaryStatus rdf:type owl:Class ;
               rdfs:subClassOf :ManagedSystemElement .


###  http://www.semanticweb.org/defaultuser/ontologies/2020/7/Onto-CMDB#Product
:Product rdf:type owl:Class ;
         rdfs:subClassOf :ManagedElement ;
         opla-sd:entityPosition [ opla-sd:entityPositionX "125.6208428994094"^^xsd:double ;
                                  opla-sd:entityPositionY "37.8752209545502"^^xsd:double ;
                                  rdfs:comment "This is an entity positioning annotation generated by CoModIDE (https://comodide.com/). Removing this annotation will break rendering the CoModIDE schema diagram view."@en
                                ] ;
         rdfs:comment "Product is a concrete class that aggregates PhysicalElements, SoftwareIdentity and/or other Products, and is acquired as a unit. Acquisition implies an agreement between supplier and consumer which may have implications to Product licensing, support and warranty."^^xsd:string .


###  http://www.semanticweb.org/defaultuser/ontologies/2020/7/Onto-CMDB#SPDX
:SPDX rdf:type owl:Class ;
      rdfs:subClassOf :SoftwareIdentity ;
      opla-sd:entityPosition [ opla-sd:entityPositionX "85.16352403219078"^^xsd:double ;
                               opla-sd:entityPositionY "207.63296031451327"^^xsd:double ;
                               rdfs:comment "This is an entity positioning annotation generated by CoModIDE (https://comodide.com/). Removing this annotation will break rendering the CoModIDE schema diagram view."@en
                             ] ;
      rdfs:comment "The Software Package Data Exchange® (SPDX®) specification is a standard format for communicating the components, licenses and copyrights associated with a software package. The need to identify the license for open source software is critical for both reporting purposes and license compliance."^^xsd:string .


###  http://www.semanticweb.org/defaultuser/ontologies/2020/7/Onto-CMDB#SWID
:SWID rdf:type owl:Class ;
      rdfs:subClassOf :SoftwareIdentity ;
      opla-sd:entityPosition [ opla-sd:entityPositionX "119.58813663955416"^^xsd:double ;
                               opla-sd:entityPositionY "55.419672363863306"^^xsd:double ;
                               rdfs:comment "This is an entity positioning annotation generated by CoModIDE (https://comodide.com/). Removing this annotation will break rendering the CoModIDE schema diagram view."@en
                             ] ;
      rdfs:comment "According to ISO/IEC 19770-2:2009  the SWID tag is an XML file containing authoritative identification and management information about a software product. Accurate identification of software allows organizations to support internal requirements and comply with regulatory requirements."^^xsd:string .


###  http://www.semanticweb.org/defaultuser/ontologies/2020/7/Onto-CMDB#SoftwareIdentity
:SoftwareIdentity rdf:type owl:Class ;
                  rdfs:subClassOf :ManagedSystemElement ;
                  opla-sd:entityPosition [ opla-sd:entityPositionX "42.72389493352092"^^xsd:double ;
                                           opla-sd:entityPositionY "144.5071153139528"^^xsd:double ;
                                           rdfs:comment "This is an entity positioning annotation generated by CoModIDE (https://comodide.com/). Removing this annotation will break rendering the CoModIDE schema diagram view."@en
                                         ] ;
                  rdfs:comment "SoftwareIdentity provides descriptive information about a software component for asset tracking and/or installation dependency management"^^xsd:string .


#################################################################
#    Individuals
#################################################################

###  http://www.semanticweb.org/defaultuser/ontologies/2020/7/Onto-CMDB#Application_Software
:Application_Software rdf:type owl:NamedIndividual ,
                               :Classifications .


###  http://www.semanticweb.org/defaultuser/ontologies/2020/7/Onto-CMDB#Configuration_Software
:Configuration_Software rdf:type owl:NamedIndividual ,
                                 :Classifications .


###  http://www.semanticweb.org/defaultuser/ontologies/2020/7/Onto-CMDB#Critical_failure
:Critical_failure rdf:type owl:NamedIndividual ,
                           :HealthState .


###  http://www.semanticweb.org/defaultuser/ontologies/2020/7/Onto-CMDB#Diagnostic_Software
:Diagnostic_Software rdf:type owl:NamedIndividual ,
                              :Classifications .


###  http://www.semanticweb.org/defaultuser/ontologies/2020/7/Onto-CMDB#Dormant
:Dormant rdf:type owl:NamedIndividual ,
                  :OperatingStatus .


###  http://www.semanticweb.org/defaultuser/ontologies/2020/7/Onto-CMDB#Driver
:Driver rdf:type owl:NamedIndividual ,
                 :Classifications .


###  http://www.semanticweb.org/defaultuser/ontologies/2020/7/Onto-CMDB#Error
:Error rdf:type owl:NamedIndividual ,
                :PrimaryStatus .


###  http://www.semanticweb.org/defaultuser/ontologies/2020/7/Onto-CMDB#Firmware
:Firmware rdf:type owl:NamedIndividual ,
                   :Classifications .


###  http://www.semanticweb.org/defaultuser/ontologies/2020/7/Onto-CMDB#In_Service
:In_Service rdf:type owl:NamedIndividual ,
                     :OperatingStatus .


###  http://www.semanticweb.org/defaultuser/ontologies/2020/7/Onto-CMDB#In_Test
:In_Test rdf:type owl:NamedIndividual ,
                  :OperatingStatus .


###  http://www.semanticweb.org/defaultuser/ontologies/2020/7/Onto-CMDB#Instrumentation
:Instrumentation rdf:type owl:NamedIndividual ,
                          :Classifications .


###  http://www.semanticweb.org/defaultuser/ontologies/2020/7/Onto-CMDB#Major_failure
:Major_failure rdf:type owl:NamedIndividual ,
                        :HealthState .


###  http://www.semanticweb.org/defaultuser/ontologies/2020/7/Onto-CMDB#Middleware
:Middleware rdf:type owl:NamedIndividual ,
                     :Classifications .


###  http://www.semanticweb.org/defaultuser/ontologies/2020/7/Onto-CMDB#Migrating
:Migrating rdf:type owl:NamedIndividual ,
                    :OperatingStatus .


###  http://www.semanticweb.org/defaultuser/ontologies/2020/7/Onto-CMDB#Minor_failure
:Minor_failure rdf:type owl:NamedIndividual ,
                        :HealthState .


###  http://www.semanticweb.org/defaultuser/ontologies/2020/7/Onto-CMDB#Non-recoverable_error
:Non-recoverable_error rdf:type owl:NamedIndividual ,
                                :HealthState .


###  http://www.semanticweb.org/defaultuser/ontologies/2020/7/Onto-CMDB#None
:None rdf:type owl:NamedIndividual ,
               :OperatingStatus .


###  http://www.semanticweb.org/defaultuser/ontologies/2020/7/Onto-CMDB#OK
:OK rdf:type owl:NamedIndividual ,
             :HealthState ,
             :PrimaryStatus .


###  http://www.semanticweb.org/defaultuser/ontologies/2020/7/Onto-CMDB#Operating_System
:Operating_System rdf:type owl:NamedIndividual ,
                           :Classifications .


###  http://www.semanticweb.org/defaultuser/ontologies/2020/7/Onto-CMDB#Other
:Other rdf:type owl:NamedIndividual ,
                :Classifications .


###  http://www.semanticweb.org/defaultuser/ontologies/2020/7/Onto-CMDB#Servicing
:Servicing rdf:type owl:NamedIndividual ,
                    :OperatingStatus .


###  http://www.semanticweb.org/defaultuser/ontologies/2020/7/Onto-CMDB#Software_Bundle
:Software_Bundle rdf:type owl:NamedIndividual ,
                          :Classifications .


###  http://www.semanticweb.org/defaultuser/ontologies/2020/7/Onto-CMDB#Transitioning
:Transitioning rdf:type owl:NamedIndividual ,
                        :OperatingStatus .


###  http://www.semanticweb.org/defaultuser/ontologies/2020/7/Onto-CMDB#Unknown
:Unknown rdf:type owl:NamedIndividual ,
                  :HealthState ,
                  :PrimaryStatus .


###  http://www.semanticweb.org/defaultuser/ontologies/2020/7/Onto-CMDB#BIOS/FCode
<http://www.semanticweb.org/defaultuser/ontologies/2020/7/Onto-CMDB#BIOS/FCode> rdf:type owl:NamedIndividual ,
                                                                                         :Classifications .


###  http://www.semanticweb.org/defaultuser/ontologies/2020/7/Onto-CMDB#Degraded/Warning
<http://www.semanticweb.org/defaultuser/ontologies/2020/7/Onto-CMDB#Degraded/Warning> rdf:type owl:NamedIndividual ,
                                                                                               :HealthState ,
                                                                                               :PrimaryStatus .


###  http://www.semanticweb.org/defaultuser/ontologies/2020/7/Onto-CMDB#Support/Service_Pack
<http://www.semanticweb.org/defaultuser/ontologies/2020/7/Onto-CMDB#Support/Service_Pack> rdf:type owl:NamedIndividual ,
                                                                                                   :Classifications .


[ ontodebug:axiom "hasProduct Range ManagedElement"^^xsd:string ;
  ontodebug:type "true"^^xsd:boolean
] .

[ ontodebug:axiom "hasProduct Range ManagedSystemElement"^^xsd:string ;
   ontodebug:type "true"^^xsd:boolean
 ] .

[ ontodebug:axiom "hasProduct Range PhysicalElement"^^xsd:string ;
   ontodebug:type "true"^^xsd:boolean
 ] .

[ ontodebug:axiom "hasProduct Range SPDX"^^xsd:string ;
   ontodebug:type "true"^^xsd:boolean
 ] .

[ ontodebug:axiom "FRU DisjointWith ManagedSystemElement"^^xsd:string ;
   ontodebug:type "true"^^xsd:boolean
 ] .

[ ontodebug:axiom "ManagedSystemElement DisjointWith Product"^^xsd:string ;
   ontodebug:type "true"^^xsd:boolean
 ] .

[ ontodebug:axiom "hasLocation Range SoftwareIdentity"^^xsd:string ;
   ontodebug:type "false"^^xsd:boolean
 ] .

[ ontodebug:axiom "hasName Domain ManagedElement"^^xsd:string ;
   ontodebug:type "true"^^xsd:boolean
 ] .

[ ontodebug:axiom "WarrantyDuration Domain SoftwareIdentity"^^xsd:string ;
   ontodebug:type "false"^^xsd:boolean
 ] .

[ ontodebug:axiom "Product DisjointWith SoftwareIdentity"^^xsd:string ;
   ontodebug:type "true"^^xsd:boolean
 ] .

[ ontodebug:axiom "WarrantyDuration Domain SPDX"^^xsd:string ;
   ontodebug:type "false"^^xsd:boolean
 ] .

[ ontodebug:axiom "hasProduct Range SoftwareIdentity"^^xsd:string ;
   ontodebug:type "true"^^xsd:boolean
 ] .

[ ontodebug:axiom "hasProduct Range FRU"^^xsd:string ;
   ontodebug:type "true"^^xsd:boolean
 ] .

[ ontodebug:axiom "hasFRU Range Product"^^xsd:string ;
   ontodebug:type "false"^^xsd:boolean
 ] .

[ ontodebug:axiom "Manufacturer Domain SoftwareIdentity"^^xsd:string ;
   ontodebug:type "false"^^xsd:boolean
 ] .

[ ontodebug:axiom "Location SubClassOf ManagedSystemElement"^^xsd:string ;
   ontodebug:type "false"^^xsd:boolean
 ] .

[ ontodebug:axiom "Classifications SubClassOf Product"^^xsd:string ;
   ontodebug:type "false"^^xsd:boolean
 ] .

[ ontodebug:axiom "Manufacturer Domain ManagedElement"^^xsd:string ;
   ontodebug:type "true"^^xsd:boolean
 ] .

[ ontodebug:axiom "Unknown Type Classifications"^^xsd:string ;
   ontodebug:type "true"^^xsd:boolean
 ] .

[ ontodebug:axiom "FRU and Product SubClassOf ManagedElement"^^xsd:string ;
   ontodebug:type "true"^^xsd:boolean
 ] .

[ ontodebug:axiom "Classifications DisjointWith OperatingStatus"^^xsd:string ;
   ontodebug:type "true"^^xsd:boolean
 ] .

[ ontodebug:axiom "SPDX SubClassOf ManagedSystemElement"^^xsd:string ;
   ontodebug:type "true"^^xsd:boolean
 ] .

[ ontodebug:axiom "OperatingStatus DisjointWith SoftwareIdentity"^^xsd:string ;
   ontodebug:type "true"^^xsd:boolean
 ] .

[ ontodebug:axiom "hasName Domain ManagedSystemElement"^^xsd:string ;
   ontodebug:type "true"^^xsd:boolean
 ] .

[ ontodebug:axiom "FRU SubClassOf ManagedSystemElement"^^xsd:string ;
   ontodebug:type "false"^^xsd:boolean
 ] .

[ ontodebug:axiom "SPDX EquivalentTo SWID"^^xsd:string ;
   ontodebug:type "false"^^xsd:boolean
 ] .

[ ontodebug:axiom "FRU DisjointWith SPDX"^^xsd:string ;
   ontodebug:type "true"^^xsd:boolean
 ] .

[ ontodebug:axiom "Location DisjointWith ManagedSystemElement"^^xsd:string ;
   ontodebug:type "true"^^xsd:boolean
 ] .

[ ontodebug:axiom "OperatingStatus Domain PhysicalElement"^^xsd:string ;
   ontodebug:type "true"^^xsd:boolean
 ] .

[ ontodebug:axiom "Product SubClassOf ManagedSystemElement"^^xsd:string ;
   ontodebug:type "false"^^xsd:boolean
 ] .

[ ontodebug:axiom "Caption Domain Location"^^xsd:string ;
   ontodebug:type "true"^^xsd:boolean
 ] .

[ ontodebug:axiom "hasFRU Range FRU"^^xsd:string ;
   ontodebug:type "true"^^xsd:boolean
 ] .

[ ontodebug:axiom "Family Domain FRU"^^xsd:string ;
   ontodebug:type "false"^^xsd:boolean
 ] .

[ ontodebug:axiom "hasFRU Domain Product"^^xsd:string ;
   ontodebug:type "false"^^xsd:boolean
 ] .

[ ontodebug:axiom "Caption Domain FRU"^^xsd:string ;
   ontodebug:type "true"^^xsd:boolean
 ] .

[ ontodebug:axiom "Location SubClassOf ManagedSystemElement"^^xsd:string ;
   ontodebug:type "false"^^xsd:boolean
 ] .

[ ontodebug:axiom "hasFRU Range Product"^^xsd:string ;
   ontodebug:type "false"^^xsd:boolean
 ] .

[ ontodebug:axiom "Manufacturer Domain ManagedElement"^^xsd:string ;
   ontodebug:type "true"^^xsd:boolean
 ] .

[ ontodebug:axiom "Product SubClassOf ManagedSystemElement"^^xsd:string ;
   ontodebug:type "false"^^xsd:boolean
 ] .

[ ontodebug:axiom "hasName Domain ManagedElement"^^xsd:string ;
   ontodebug:type "true"^^xsd:boolean
 ] .

[ ontodebug:axiom "hasName Domain ManagedSystemElement"^^xsd:string ;
   ontodebug:type "true"^^xsd:boolean
 ] .

[ ontodebug:axiom "Manufacturer Domain SoftwareIdentity"^^xsd:string ;
   ontodebug:type "false"^^xsd:boolean
 ] .

[ ontodebug:axiom "hasName Domain ManagedElement"^^xsd:string ;
   ontodebug:type "true"^^xsd:boolean
 ] .

[ ontodebug:axiom "hasName Domain ManagedSystemElement"^^xsd:string ;
   ontodebug:type "true"^^xsd:boolean
 ] .

[ ontodebug:axiom "FRU SubClassOf ManagedSystemElement"^^xsd:string ;
   ontodebug:type "false"^^xsd:boolean
 ] .

[ ontodebug:axiom "hasName Domain ManagedSystemElement"^^xsd:string ;
   ontodebug:type "true"^^xsd:boolean
 ] .

[ ontodebug:axiom "hasName Domain ManagedSystemElement"^^xsd:string ;
   ontodebug:type "true"^^xsd:boolean
 ] .

[ ontodebug:axiom "FRU SubClassOf ManagedSystemElement"^^xsd:string ;
   ontodebug:type "false"^^xsd:boolean
 ] .

[ ontodebug:axiom "Location DisjointWith ManagedSystemElement"^^xsd:string ;
   ontodebug:type "true"^^xsd:boolean
 ] .

[ ontodebug:axiom "hasFRU Range FRU"^^xsd:string ;
   ontodebug:type "true"^^xsd:boolean
 ] .

[ ontodebug:axiom "hasName Domain ManagedSystemElement"^^xsd:string ;
   ontodebug:type "true"^^xsd:boolean
 ] .

[ ontodebug:axiom "Product DisjointWith SoftwareIdentity"^^xsd:string ;
   ontodebug:type "true"^^xsd:boolean
 ] .

[ ontodebug:axiom "WarrantyDuration Domain SPDX"^^xsd:string ;
   ontodebug:type "false"^^xsd:boolean
 ] .

[ ontodebug:axiom "Classifications SubClassOf Product"^^xsd:string ;
   ontodebug:type "false"^^xsd:boolean
 ] .

[ ontodebug:axiom "Unknown Type Classifications"^^xsd:string ;
   ontodebug:type "true"^^xsd:boolean
 ] .

[ ontodebug:axiom "WarrantyDuration Domain SoftwareIdentity"^^xsd:string ;
   ontodebug:type "false"^^xsd:boolean
 ] .

[ ontodebug:axiom "FRU SubClassOf ManagedSystemElement"^^xsd:string ;
   ontodebug:type "false"^^xsd:boolean
 ] .

[ ontodebug:axiom "hasFRU Range FRU"^^xsd:string ;
   ontodebug:type "true"^^xsd:boolean
 ] .

[ ontodebug:axiom "FRU SubClassOf ManagedSystemElement"^^xsd:string ;
   ontodebug:type "false"^^xsd:boolean
 ] .

[ ontodebug:axiom "hasFRU Domain Product"^^xsd:string ;
   ontodebug:type "false"^^xsd:boolean
 ] .

[ ontodebug:axiom "Location SubClassOf ManagedSystemElement"^^xsd:string ;
   ontodebug:type "false"^^xsd:boolean
 ] .

[ ontodebug:axiom "hasFRU Domain Product"^^xsd:string ;
   ontodebug:type "false"^^xsd:boolean
 ] .

[ ontodebug:axiom "FRU DisjointWith ManagedSystemElement"^^xsd:string ;
   ontodebug:type "true"^^xsd:boolean
 ] .

[ ontodebug:axiom "FRU DisjointWith ManagedSystemElement"^^xsd:string ;
   ontodebug:type "true"^^xsd:boolean
 ] .

[ ontodebug:axiom "hasName Domain ManagedElement"^^xsd:string ;
   ontodebug:type "true"^^xsd:boolean
 ] .

[ ontodebug:axiom "hasFRU Range FRU"^^xsd:string ;
   ontodebug:type "true"^^xsd:boolean
 ] .

[ ontodebug:axiom "hasName Domain ManagedElement"^^xsd:string ;
   ontodebug:type "true"^^xsd:boolean
 ] .

[ ontodebug:axiom "Family Domain FRU"^^xsd:string ;
   ontodebug:type "false"^^xsd:boolean
 ] .

[ ontodebug:axiom "hasName Domain ManagedSystemElement"^^xsd:string ;
   ontodebug:type "true"^^xsd:boolean
 ] .

[ ontodebug:axiom "hasFRU Range FRU"^^xsd:string ;
   ontodebug:type "true"^^xsd:boolean
 ] .

[ ontodebug:axiom "ManagedSystemElement DisjointWith Product"^^xsd:string ;
   ontodebug:type "true"^^xsd:boolean
 ] .

[ ontodebug:axiom "Classifications DisjointWith OperatingStatus"^^xsd:string ;
   ontodebug:type "true"^^xsd:boolean
 ] .

[ ontodebug:axiom "OperatingStatus DisjointWith SoftwareIdentity"^^xsd:string ;
   ontodebug:type "true"^^xsd:boolean
 ] .

[ ontodebug:axiom "hasName Domain ManagedElement"^^xsd:string ;
   ontodebug:type "true"^^xsd:boolean
 ] .

[ ontodebug:axiom "OperatingStatus Domain PhysicalElement"^^xsd:string ;
   ontodebug:type "true"^^xsd:boolean
 ] .

[ ontodebug:axiom "ManagedSystemElement DisjointWith Product"^^xsd:string ;
   ontodebug:type "true"^^xsd:boolean
 ] .

[ ontodebug:axiom "Caption Domain Location"^^xsd:string ;
   ontodebug:type "true"^^xsd:boolean
 ] .

[ ontodebug:axiom "FRU SubClassOf ManagedSystemElement"^^xsd:string ;
   ontodebug:type "false"^^xsd:boolean
 ] .

[ ontodebug:axiom "Location DisjointWith ManagedSystemElement"^^xsd:string ;
   ontodebug:type "true"^^xsd:boolean
 ] .

[ ontodebug:axiom "hasName Domain ManagedElement"^^xsd:string ;
   ontodebug:type "true"^^xsd:boolean
 ] .

[ ontodebug:axiom "hasFRU Range FRU"^^xsd:string ;
   ontodebug:type "true"^^xsd:boolean
 ] .

[ ontodebug:axiom "Product SubClassOf ManagedSystemElement"^^xsd:string ;
   ontodebug:type "false"^^xsd:boolean
 ] .

[ ontodebug:axiom "hasFRU Domain Product"^^xsd:string ;
   ontodebug:type "false"^^xsd:boolean
 ] .

[ ontodebug:axiom "Product SubClassOf ManagedSystemElement"^^xsd:string ;
   ontodebug:type "false"^^xsd:boolean
 ] .

[ ontodebug:axiom "Location DisjointWith ManagedSystemElement"^^xsd:string ;
   ontodebug:type "true"^^xsd:boolean
 ] .

[ ontodebug:axiom "hasFRU Domain Product"^^xsd:string ;
   ontodebug:type "false"^^xsd:boolean
 ] .

[ ontodebug:axiom "Location DisjointWith ManagedSystemElement"^^xsd:string ;
   ontodebug:type "true"^^xsd:boolean
 ] .

[ ontodebug:axiom "ManagedSystemElement DisjointWith Product"^^xsd:string ;
   ontodebug:type "true"^^xsd:boolean
 ] .

[ ontodebug:axiom "hasName Domain ManagedSystemElement"^^xsd:string ;
   ontodebug:type "true"^^xsd:boolean
 ] .

[ ontodebug:axiom "Location SubClassOf ManagedSystemElement"^^xsd:string ;
   ontodebug:type "false"^^xsd:boolean
 ] .

[ ontodebug:axiom "Location SubClassOf ManagedSystemElement"^^xsd:string ;
   ontodebug:type "false"^^xsd:boolean
 ] .

[ ontodebug:axiom "hasName Domain ManagedSystemElement"^^xsd:string ;
   ontodebug:type "true"^^xsd:boolean
 ] .

[ ontodebug:axiom "hasName Domain ManagedElement"^^xsd:string ;
   ontodebug:type "true"^^xsd:boolean
 ] .

[ ontodebug:axiom "Product SubClassOf ManagedSystemElement"^^xsd:string ;
   ontodebug:type "false"^^xsd:boolean
 ] .

[ ontodebug:axiom "hasName Domain ManagedSystemElement"^^xsd:string ;
   ontodebug:type "true"^^xsd:boolean
 ] .

[ ontodebug:axiom "hasName Domain ManagedSystemElement"^^xsd:string ;
   ontodebug:type "true"^^xsd:boolean
 ] .

[ ontodebug:axiom "hasName Domain ManagedElement"^^xsd:string ;
   ontodebug:type "true"^^xsd:boolean
 ] .

[ ontodebug:axiom "Location DisjointWith ManagedSystemElement"^^xsd:string ;
   ontodebug:type "true"^^xsd:boolean
 ] .

[ ontodebug:axiom "FRU DisjointWith ManagedSystemElement"^^xsd:string ;
   ontodebug:type "true"^^xsd:boolean
 ] .

[ ontodebug:axiom "Location SubClassOf ManagedSystemElement"^^xsd:string ;
   ontodebug:type "false"^^xsd:boolean
 ] .

[ ontodebug:axiom "hasName Domain ManagedSystemElement"^^xsd:string ;
   ontodebug:type "true"^^xsd:boolean
 ] .

[ ontodebug:axiom "hasName Domain ManagedElement"^^xsd:string ;
   ontodebug:type "true"^^xsd:boolean
 ] .

[ ontodebug:axiom "Product SubClassOf ManagedSystemElement"^^xsd:string ;
   ontodebug:type "false"^^xsd:boolean
 ] .

[ ontodebug:axiom "hasName Domain ManagedElement"^^xsd:string ;
   ontodebug:type "true"^^xsd:boolean
 ] .

[ ontodebug:axiom "hasName Domain ManagedSystemElement"^^xsd:string ;
   ontodebug:type "true"^^xsd:boolean
 ] .

[ ontodebug:axiom "hasName Domain ManagedElement"^^xsd:string ;
   ontodebug:type "true"^^xsd:boolean
 ] .

[ ontodebug:axiom "FRU and Product SubClassOf ManagedElement"^^xsd:string ;
   ontodebug:type "true"^^xsd:boolean
 ] .

[ ontodebug:axiom "FRU SubClassOf ManagedSystemElement"^^xsd:string ;
   ontodebug:type "false"^^xsd:boolean
 ] .

[ ontodebug:axiom "SPDX SubClassOf ManagedSystemElement"^^xsd:string ;
   ontodebug:type "true"^^xsd:boolean
 ] .

[ ontodebug:axiom "hasName Domain ManagedSystemElement"^^xsd:string ;
   ontodebug:type "true"^^xsd:boolean
 ] .

[ ontodebug:axiom "hasName Domain ManagedElement"^^xsd:string ;
   ontodebug:type "true"^^xsd:boolean
 ] .

[ ontodebug:axiom "hasName Domain ManagedSystemElement"^^xsd:string ;
   ontodebug:type "true"^^xsd:boolean
 ] .

[ ontodebug:axiom "FRU DisjointWith ManagedSystemElement"^^xsd:string ;
   ontodebug:type "true"^^xsd:boolean
 ] .

[ ontodebug:axiom "hasFRU Domain Product"^^xsd:string ;
   ontodebug:type "false"^^xsd:boolean
 ] .

[ ontodebug:axiom "FRU DisjointWith ManagedSystemElement"^^xsd:string ;
   ontodebug:type "true"^^xsd:boolean
 ] .

[ ontodebug:axiom "ManagedSystemElement DisjointWith Product"^^xsd:string ;
   ontodebug:type "true"^^xsd:boolean
 ] .

[ ontodebug:axiom "Location DisjointWith ManagedSystemElement"^^xsd:string ;
   ontodebug:type "true"^^xsd:boolean
 ] .

[ ontodebug:axiom "hasName Domain ManagedElement"^^xsd:string ;
   ontodebug:type "true"^^xsd:boolean
 ] .

[ ontodebug:axiom "Product SubClassOf ManagedSystemElement"^^xsd:string ;
   ontodebug:type "false"^^xsd:boolean
 ] .

[ ontodebug:axiom "hasFRU Range FRU"^^xsd:string ;
   ontodebug:type "true"^^xsd:boolean
 ] .

[ ontodebug:axiom "hasFRU Domain Product"^^xsd:string ;
   ontodebug:type "false"^^xsd:boolean
 ] .

[ ontodebug:axiom "hasName Domain ManagedElement"^^xsd:string ;
   ontodebug:type "true"^^xsd:boolean
 ] .

[ ontodebug:axiom "FRU SubClassOf ManagedSystemElement"^^xsd:string ;
   ontodebug:type "false"^^xsd:boolean
 ] .

[ ontodebug:axiom "hasName Domain ManagedElement"^^xsd:string ;
   ontodebug:type "true"^^xsd:boolean
 ] .

[ ontodebug:axiom "FRU DisjointWith ManagedSystemElement"^^xsd:string ;
   ontodebug:type "true"^^xsd:boolean
 ] .

[ ontodebug:axiom "Location DisjointWith ManagedSystemElement"^^xsd:string ;
   ontodebug:type "true"^^xsd:boolean
 ] .

[ ontodebug:axiom "Product SubClassOf ManagedSystemElement"^^xsd:string ;
   ontodebug:type "false"^^xsd:boolean
 ] .

[ ontodebug:axiom "ManagedSystemElement DisjointWith Product"^^xsd:string ;
   ontodebug:type "true"^^xsd:boolean
 ] .

[ ontodebug:axiom "hasName Domain ManagedSystemElement"^^xsd:string ;
   ontodebug:type "true"^^xsd:boolean
 ] .

[ ontodebug:axiom "hasName Domain ManagedElement"^^xsd:string ;
   ontodebug:type "true"^^xsd:boolean
 ] .

[ ontodebug:axiom "hasName Domain ManagedSystemElement"^^xsd:string ;
   ontodebug:type "true"^^xsd:boolean
 ] .

[ ontodebug:axiom "hasName Domain ManagedSystemElement"^^xsd:string ;
   ontodebug:type "true"^^xsd:boolean
 ] .

[ ontodebug:axiom "hasName Domain ManagedElement"^^xsd:string ;
   ontodebug:type "true"^^xsd:boolean
 ] .

[ ontodebug:axiom "ManagedSystemElement DisjointWith Product"^^xsd:string ;
   ontodebug:type "true"^^xsd:boolean
 ] .

[ ontodebug:axiom "hasName Domain ManagedSystemElement"^^xsd:string ;
   ontodebug:type "true"^^xsd:boolean
 ] .

[ ontodebug:axiom "hasName Domain ManagedElement"^^xsd:string ;
   ontodebug:type "true"^^xsd:boolean
 ] .

[ ontodebug:axiom "Manufacturer Domain SoftwareIdentity"^^xsd:string ;
   ontodebug:type "false"^^xsd:boolean
 ] .

[ ontodebug:axiom "hasName Domain ManagedElement"^^xsd:string ;
   ontodebug:type "true"^^xsd:boolean
 ] .

[ ontodebug:axiom "Caption Domain FRU"^^xsd:string ;
   ontodebug:type "true"^^xsd:boolean
 ] .

[ ontodebug:axiom "hasName Domain ManagedSystemElement"^^xsd:string ;
   ontodebug:type "true"^^xsd:boolean
 ] .

[ ontodebug:axiom "SPDX EquivalentTo SWID"^^xsd:string ;
   ontodebug:type "false"^^xsd:boolean
 ] .

[ ontodebug:axiom "FRU DisjointWith SPDX"^^xsd:string ;
   ontodebug:type "true"^^xsd:boolean
 ] .

[ ontodebug:axiom "Location SubClassOf ManagedSystemElement"^^xsd:string ;
   ontodebug:type "false"^^xsd:boolean
 ] .

[ ontodebug:axiom "FRU and Product SubClassOf ManagedElement"^^xsd:string ;
   ontodebug:type "true"^^xsd:boolean
 ] .

[ ontodebug:axiom "SPDX SubClassOf ManagedSystemElement"^^xsd:string ;
   ontodebug:type "true"^^xsd:boolean
 ] .

[ ontodebug:axiom "Manufacturer Domain ManagedElement"^^xsd:string ;
   ontodebug:type "true"^^xsd:boolean
 ] .

[ ontodebug:axiom "hasProduct Range SPDX"^^xsd:string ;
   ontodebug:type "true"^^xsd:boolean
 ] .

[ ontodebug:axiom "hasProduct Range SoftwareIdentity"^^xsd:string ;
   ontodebug:type "true"^^xsd:boolean
 ] .

[ ontodebug:axiom "hasProduct Range FRU"^^xsd:string ;
   ontodebug:type "true"^^xsd:boolean
 ] .

[ ontodebug:axiom "hasLocation Range SoftwareIdentity"^^xsd:string ;
   ontodebug:type "false"^^xsd:boolean
 ] .

[ ontodebug:axiom "hasProduct Range ManagedElement"^^xsd:string ;
   ontodebug:type "true"^^xsd:boolean
 ] .

[ ontodebug:axiom "hasProduct Range ManagedSystemElement"^^xsd:string ;
   ontodebug:type "true"^^xsd:boolean
 ] .

[ ontodebug:axiom "hasProduct Range PhysicalElement"^^xsd:string ;
   ontodebug:type "true"^^xsd:boolean
 ] .

#################################################################
#    Annotations
#################################################################

:PrimaryStatus rdfs:comment """PrimaryStatus provides a high level status value, intended to align with Red-Yellow-Green type representation of status. It should be used in conjunction with DetailedStatus to provide high level and detailed health status of the ManagedElement and its subcomponents. PrimaryStatus consists of one of the following values: Unknown, OK, Degraded or Error. \"Unknown\" indicates the implementation is in general capable of returning this property, but is unable to do so at this time. \"OK\" indicates the ManagedElement is functioning normally. \"Degraded\" indicates the ManagedElement is functioning below normal. \"Error\" indicates the ManagedElement is in an Error condition.

Values:Unknown, OK, Degraded, Error"""^^xsd:string .


#################################################################
#    General axioms
#################################################################

[ rdf:type owl:AllDisjointClasses ;
  owl:members ( :FRU
                :Location
                :ManagedSystemElement
                :Product
              )
] .


[ rdf:type owl:AllDisjointClasses ;
  owl:members ( :OperatingStatus
                :PhysicalElement
                :SoftwareIdentity
              )
] .


###  Generated by the OWL API (version 4.5.9.2019-02-01T07:24:44Z) https://github.com/owlcs/owlapi
