@prefix : <http://www.semanticweb.org/defaultuser/ontologies/2020/7/Onto-CMDB#> .
@prefix owl: <http://www.w3.org/2002/07/owl#> .
@prefix rdf: <http://www.w3.org/1999/02/22-rdf-syntax-ns#> .
@prefix xml: <http://www.w3.org/XML/1998/namespace> .
@prefix xsd: <http://www.w3.org/2001/XMLSchema#> .
@prefix rdfs: <http://www.w3.org/2000/01/rdf-schema#> .
@prefix opla-sd: <http://ontologydesignpatterns.org/opla-sd#> .
@prefix ontodebug: <http://ainf.aau.at/ontodebug#> .
@base <http://www.semanticweb.org/defaultuser/ontologies/2020/7/Onto-CMDB> .

<http://www.semanticweb.org/defaultuser/ontologies/2020/7/Onto-CMDB> rdf:type owl:Ontology ;
                                                                      ontodebug:testCase [ ontodebug:axiom "hasFRU Range FRU"^^xsd:string ;
                                                                                           ontodebug:type "true"^^xsd:boolean
                                                                                         ] ,
                                                                                         [ ontodebug:axiom "hasName Domain ManagedSystemElement"^^xsd:string ;
                                                                                           ontodebug:type "true"^^xsd:boolean
                                                                                         ] ,
                                                                                         [ ontodebug:axiom "WarrantyDuration Domain SoftwareIdentity"^^xsd:string ;
                                                                                           ontodebug:type "false"^^xsd:boolean
                                                                                         ] ,
                                                                                         [ ontodebug:axiom "OperatingStatus DisjointWith SoftwareIdentity"^^xsd:string ;
                                                                                           ontodebug:type "true"^^xsd:boolean
                                                                                         ] ,
                                                                                         [ ontodebug:axiom "OperatingStatus Domain PhysicalElement"^^xsd:string ;
                                                                                           ontodebug:type "true"^^xsd:boolean
                                                                                         ] ,
                                                                                         [ ontodebug:axiom "Manufacturer Domain ManagedElement"^^xsd:string ;
                                                                                           ontodebug:type "true"^^xsd:boolean
                                                                                         ] ,
                                                                                         [ ontodebug:axiom "CISCO_CATALYST_3750 Caption \"Cisco Catalyst 3750\"^^string"^^xsd:string ;
                                                                                           ontodebug:type "true"^^xsd:boolean
                                                                                         ] ,
                                                                                         [ ontodebug:axiom "Classifications DisjointWith OperatingStatus"^^xsd:string ;
                                                                                           ontodebug:type "true"^^xsd:boolean
                                                                                         ] ,
                                                                                         [ ontodebug:axiom "SPDX SubClassOf ManagedSystemElement"^^xsd:string ;
                                                                                           ontodebug:type "true"^^xsd:boolean
                                                                                         ] ,
                                                                                         [ ontodebug:axiom "SoftwareCreator Domain PhysicalElement"^^xsd:string ;
                                                                                           ontodebug:type "false"^^xsd:boolean
                                                                                         ] ,
                                                                                         [ ontodebug:axiom "FRU SubClassOf ManagedSystemElement"^^xsd:string ;
                                                                                           ontodebug:type "false"^^xsd:boolean
                                                                                         ] ,
                                                                                         [ ontodebug:axiom "SerialNumber Domain PhysicalElement"^^xsd:string ;
                                                                                           ontodebug:type "true"^^xsd:boolean
                                                                                         ] ,
                                                                                         [ ontodebug:axiom "SPDX EquivalentTo SWID"^^xsd:string ;
                                                                                           ontodebug:type "false"^^xsd:boolean
                                                                                         ] ,
                                                                                         [ ontodebug:axiom "Manufacturer Domain SoftwareIdentity"^^xsd:string ;
                                                                                           ontodebug:type "false"^^xsd:boolean
                                                                                         ] ,
                                                                                         [ ontodebug:axiom "Name Domain ManagedElement"^^xsd:string ;
                                                                                           ontodebug:type "true"^^xsd:boolean
                                                                                         ] ,
                                                                                         [ ontodebug:axiom "Unknown Type Classifications"^^xsd:string ;
                                                                                           ontodebug:type "true"^^xsd:boolean
                                                                                         ] ,
                                                                                         [ ontodebug:axiom "Family Domain FRU"^^xsd:string ;
                                                                                           ontodebug:type "false"^^xsd:boolean
                                                                                         ] ,
                                                                                         [ ontodebug:axiom "hasName Domain ManagedElement"^^xsd:string ;
                                                                                           ontodebug:type "true"^^xsd:boolean
                                                                                         ] ,
                                                                                         [ ontodebug:axiom "Classifications SubClassOf Product"^^xsd:string ;
                                                                                           ontodebug:type "false"^^xsd:boolean
                                                                                         ] ,
                                                                                         [ ontodebug:axiom "hasLocation Range SoftwareIdentity"^^xsd:string ;
                                                                                           ontodebug:type "false"^^xsd:boolean
                                                                                         ] ,
                                                                                         [ ontodebug:axiom "WarrantyDuration Domain SPDX"^^xsd:string ;
                                                                                           ontodebug:type "false"^^xsd:boolean
                                                                                         ] ,
                                                                                         [ ontodebug:axiom "hasProduct Range ManagedElement"^^xsd:string ;
                                                                                           ontodebug:type "true"^^xsd:boolean
                                                                                         ] ,
                                                                                         [ ontodebug:axiom "Name Domain PhysicalElement"^^xsd:string ;
                                                                                           ontodebug:type "true"^^xsd:boolean
                                                                                         ] .

#################################################################
#    Annotation properties
#################################################################

###  http://ainf.aau.at/ontodebug#axiom
ontodebug:axiom rdf:type owl:AnnotationProperty ;
                rdfs:subPropertyOf ontodebug:testCase .


###  http://ainf.aau.at/ontodebug#testCase
ontodebug:testCase rdf:type owl:AnnotationProperty .


###  http://ainf.aau.at/ontodebug#type
ontodebug:type rdf:type owl:AnnotationProperty ;
               rdfs:subPropertyOf ontodebug:testCase .


###  http://ontologydesignpatterns.org/opla-sd#entityPosition
opla-sd:entityPosition rdf:type owl:AnnotationProperty .


###  http://ontologydesignpatterns.org/opla-sd#entityPositionX
opla-sd:entityPositionX rdf:type owl:AnnotationProperty .


###  http://ontologydesignpatterns.org/opla-sd#entityPositionY
opla-sd:entityPositionY rdf:type owl:AnnotationProperty .


#################################################################
#    Object Properties
#################################################################

###  http://www.semanticweb.org/defaultuser/ontologies/2020/7/Onto-CMDB#hasFRU
:hasFRU rdf:type owl:ObjectProperty ;
        rdfs:subPropertyOf owl:topObjectProperty ;
        rdfs:domain :ManagedElement ;
        rdfs:range :FRU ;
        owl:propertyDisjointWith :hasLocation ,
                                 :hasManagedSystemElement ,
                                 :hasProduct ,
                                 :hasSoftwareIdentity .


###  http://www.semanticweb.org/defaultuser/ontologies/2020/7/Onto-CMDB#hasLocation
:hasLocation rdf:type owl:ObjectProperty ;
             rdfs:domain :ManagedSystemElement ;
             rdfs:range :Location .


###  http://www.semanticweb.org/defaultuser/ontologies/2020/7/Onto-CMDB#hasManagedSystemElement
:hasManagedSystemElement rdf:type owl:ObjectProperty ;
                         rdfs:domain :ManagedElement ;
                         rdfs:range :ManagedSystemElement ;
                         owl:propertyDisjointWith :hasProduct .


###  http://www.semanticweb.org/defaultuser/ontologies/2020/7/Onto-CMDB#hasPhysicalElement
:hasPhysicalElement rdf:type owl:ObjectProperty ;
                    rdfs:domain :ManagedSystemElement ;
                    rdfs:range :PhysicalElement ;
                    owl:propertyDisjointWith :hasSoftwareIdentity .


###  http://www.semanticweb.org/defaultuser/ontologies/2020/7/Onto-CMDB#hasProduct
:hasProduct rdf:type owl:ObjectProperty ;
            rdfs:domain :ManagedElement ;
            rdfs:range :Product ;
            owl:propertyDisjointWith :hasSoftwareIdentity .


###  http://www.semanticweb.org/defaultuser/ontologies/2020/7/Onto-CMDB#hasSPDX
:hasSPDX rdf:type owl:ObjectProperty ;
         rdfs:domain :SoftwareIdentity ;
         rdfs:range :SPDX .


###  http://www.semanticweb.org/defaultuser/ontologies/2020/7/Onto-CMDB#hasSWID
:hasSWID rdf:type owl:ObjectProperty ;
         rdfs:domain :SoftwareIdentity ;
         rdfs:range :SWID .


###  http://www.semanticweb.org/defaultuser/ontologies/2020/7/Onto-CMDB#hasSoftwareIdentity
:hasSoftwareIdentity rdf:type owl:ObjectProperty ;
                     rdfs:domain :ManagedSystemElement ;
                     rdfs:range :SoftwareIdentity .


#################################################################
#    Data properties
#################################################################

###  http://www.semanticweb.org/defaultuser/ontologies/2020/7/Onto-CMDB#Address
:Address rdf:type owl:DatatypeProperty ;
         rdfs:subPropertyOf owl:topDataProperty ;
         rdfs:domain :Location ;
         rdfs:range xsd:string ;
         rdfs:comment "Address is a free-form string indicating a street, building, or other type of address for the location of the PhysicalElement."^^xsd:string .


###  http://www.semanticweb.org/defaultuser/ontologies/2020/7/Onto-CMDB#Caption
:Caption rdf:type owl:DatatypeProperty ;
         rdfs:subPropertyOf owl:topDataProperty ;
         rdfs:domain :ManagedElement ;
         rdfs:range xsd:string ;
         rdfs:comment "The Caption property is a short textual description (one- line string) of the object."^^xsd:string .


###  http://www.semanticweb.org/defaultuser/ontologies/2020/7/Onto-CMDB#Description
:Description rdf:type owl:DatatypeProperty ;
             rdfs:subPropertyOf owl:topDataProperty ;
             rdfs:domain :ManagedElement ;
             rdfs:range xsd:string ;
             rdfs:comment "The Description property provides a textual description of the object."^^xsd:string .


###  http://www.semanticweb.org/defaultuser/ontologies/2020/7/Onto-CMDB#ElementName
:ElementName rdf:type owl:DatatypeProperty ;
             rdfs:subPropertyOf owl:topDataProperty ;
             rdfs:domain :ManagedElement ;
             rdfs:range xsd:string ;
             rdfs:comment "A user-friendly name for the object. This property allows each instance to define a user-friendly name in addition to its key properties, identity data, and description information. Note that the Name property of ManagedSystemElement is also defined as a user-friendly name."^^xsd:string .


###  http://www.semanticweb.org/defaultuser/ontologies/2020/7/Onto-CMDB#EntitlementRequiredIndicator
:EntitlementRequiredIndicator rdf:type owl:DatatypeProperty ;
                              rdfs:subPropertyOf owl:topDataProperty ;
                              rdfs:domain :SWID ;
                              rdfs:range xsd:boolean ;
                              rdfs:comment """Identifies whether this application needs to match up with an entitlement for a reconciliation to be considered successful. Specifies if an entitlement is required to reconcile this application. See ISO/IEC 19770-2:2009 for guidance.
Example data format:
XX = entitlement status (true = entitlement required; false = no entitlement required)"""^^xsd:string .


###  http://www.semanticweb.org/defaultuser/ontologies/2020/7/Onto-CMDB#ExtendedResourceType
:ExtendedResourceType rdf:type owl:DatatypeProperty ;
                      rdfs:subPropertyOf owl:topDataProperty ;
                      rdfs:domain :SoftwareIdentity ;
                      rdfs:range xsd:string ;
                      rdfs:comment "The binary format type of the installation package of the software."^^xsd:string .


###  http://www.semanticweb.org/defaultuser/ontologies/2020/7/Onto-CMDB#FRUNumber
:FRUNumber rdf:type owl:DatatypeProperty ;
           rdfs:subPropertyOf owl:topDataProperty ;
           rdfs:domain :FRU ;
           rdfs:range xsd:string ;
           rdfs:comment "FRU ordering information."^^xsd:string .


###  http://www.semanticweb.org/defaultuser/ontologies/2020/7/Onto-CMDB#Family
:Family rdf:type owl:DatatypeProperty ;
        rdfs:subPropertyOf owl:topDataProperty ;
        rdfs:domain :Product ;
        rdfs:range xsd:string ;
        rdfs:comment "Family that the product belongs to. A family refers to a set of products that are similar but not identical from a hardware or software point of view. Typically, a family is composed of different products, which have different configurations and pricing points. Products in the same family often have similar branding and cosmetic features."^^xsd:string .


###  http://www.semanticweb.org/defaultuser/ontologies/2020/7/Onto-CMDB#FullName
:FullName rdf:type owl:DatatypeProperty ;
          rdfs:subPropertyOf owl:topDataProperty ;
          rdfs:domain :SPDX ;
          rdfs:range xsd:string ;
          rdfs:comment "For example: MIT License or Apache License 2.0"^^xsd:string .


###  http://www.semanticweb.org/defaultuser/ontologies/2020/7/Onto-CMDB#Generation
:Generation rdf:type owl:DatatypeProperty ;
            rdfs:subPropertyOf owl:topDataProperty ;
            rdfs:domain :ManagedElement ;
            rdfs:range xsd:string ;
            rdfs:comment "Generation is an optional, monotonically increasing property that may be used to identify a particular generation of the resource represented by this class."^^xsd:string .


###  http://www.semanticweb.org/defaultuser/ontologies/2020/7/Onto-CMDB#IdentifyingNumber
:IdentifyingNumber rdf:type owl:DatatypeProperty ;
                   rdfs:subPropertyOf owl:topDataProperty ;
                   rdfs:domain :FRU ;
                   rdfs:range rdf:PlainLiteral ;
                   rdfs:comment "FRU identification such as a serial number on software or a die number on a hardware chip."^^xsd:string .


###  http://www.semanticweb.org/defaultuser/ontologies/2020/7/Onto-CMDB#InstallDate
:InstallDate rdf:type owl:DatatypeProperty ;
             rdfs:subPropertyOf owl:topDataProperty ;
             rdfs:domain :ManagedSystemElement ;
             rdfs:range xsd:dateTime ;
             rdfs:comment "A datetime value that indicates when the object was installed. Lack of a value does not indicate that the object is not installed."^^xsd:string .


###  http://www.semanticweb.org/defaultuser/ontologies/2020/7/Onto-CMDB#LargeBuildNumber
:LargeBuildNumber rdf:type owl:DatatypeProperty ;
                  rdfs:subPropertyOf owl:topDataProperty ;
                  rdfs:domain :SoftwareIdentity ;
                  rdfs:range xsd:integer ;
                  rdfs:comment "The build number of the software"^^xsd:string .


###  http://www.semanticweb.org/defaultuser/ontologies/2020/7/Onto-CMDB#MajorVersion
:MajorVersion rdf:type owl:DatatypeProperty ;
              rdfs:subPropertyOf owl:topDataProperty ;
              rdfs:domain :SoftwareIdentity ;
              rdfs:range xsd:integer ;
              rdfs:comment "The major number component of the software's version information - for example, '12' from version 12.1(3)T. This property is defined as a numeric value to allow the determination of 'newer' vs. 'older' releases. A 'newer' major release is indicated by a larger numeric value."^^xsd:string .


###  http://www.semanticweb.org/defaultuser/ontologies/2020/7/Onto-CMDB#ManufactureDate
:ManufactureDate rdf:type owl:DatatypeProperty ;
                 rdfs:subPropertyOf owl:topDataProperty ;
                 rdfs:domain :PhysicalElement ;
                 rdfs:range xsd:dateTime ;
                 rdfs:comment "The date that this PhysicalElement was manufactured"^^xsd:string .


###  http://www.semanticweb.org/defaultuser/ontologies/2020/7/Onto-CMDB#Manufacturer
:Manufacturer rdf:type owl:DatatypeProperty ;
              rdfs:subPropertyOf owl:topDataProperty ;
              rdfs:domain :PhysicalElement ;
              rdfs:range xsd:string ;
              rdfs:comment "The name of the organization responsible for producing the PhysicalElement. This organization might be the entity from whom the Element is purchased, but this is not necessarily true. The latter information is contained in the Vendor property of Product."^^xsd:string .


###  http://www.semanticweb.org/defaultuser/ontologies/2020/7/Onto-CMDB#MinorVersion
:MinorVersion rdf:type owl:DatatypeProperty ;
              rdfs:subPropertyOf owl:topDataProperty ;
              rdfs:domain :SoftwareIdentity ;
              rdfs:range xsd:integer ;
              rdfs:comment "The minor number component of the software's version information - for example, '1' from version 12.1(3)T. This property is defined as a numeric value to allow the determination of 'newer' vs. 'older' releases. A 'newer' minor release is indicated by a larger numeric value."^^xsd:string .


###  http://www.semanticweb.org/defaultuser/ontologies/2020/7/Onto-CMDB#Model
:Model rdf:type owl:DatatypeProperty ;
       rdfs:subPropertyOf owl:topDataProperty ;
       rdfs:domain :PhysicalElement ;
       rdfs:range xsd:string ;
       rdfs:comment "The name by which the PhysicalElement is generally known"^^xsd:string .


###  http://www.semanticweb.org/defaultuser/ontologies/2020/7/Onto-CMDB#Name
:Name rdf:type owl:DatatypeProperty ;
      rdfs:subPropertyOf owl:topDataProperty ;
      rdfs:domain :ManagedElement ;
      rdfs:range xsd:Name ;
      rdfs:comment "The Name property defines the label by which the object is known."^^xsd:string .


###  http://www.semanticweb.org/defaultuser/ontologies/2020/7/Onto-CMDB#Notes
:Notes rdf:type owl:DatatypeProperty ;
       rdfs:subPropertyOf owl:topDataProperty ;
       rdfs:domain :SPDX ;
       rdfs:range xsd:string ;
       rdfs:comment "Additional information about the license."^^xsd:string .


###  http://www.semanticweb.org/defaultuser/ontologies/2020/7/Onto-CMDB#OtherIdentifyingInfo
:OtherIdentifyingInfo rdf:type owl:DatatypeProperty ;
                      rdfs:subPropertyOf owl:topDataProperty ;
                      rdfs:domain :PhysicalElement ;
                      rdfs:range xsd:string ;
                      rdfs:comment "OtherIdentifyingInfo captures data in addition to Tag information. This information could be used to identify a Physical Element. One example is bar code data associated with an Element that also has an asset tag."^^xsd:string .


###  http://www.semanticweb.org/defaultuser/ontologies/2020/7/Onto-CMDB#PartNumber
:PartNumber rdf:type owl:DatatypeProperty ;
            rdfs:subPropertyOf owl:topDataProperty ;
            rdfs:domain :PhysicalElement ;
            rdfs:range xsd:string ;
            rdfs:comment "The part number assigned by the organization that is responsible for producing or manufacturing the PhysicalElement."^^xsd:string .


###  http://www.semanticweb.org/defaultuser/ontologies/2020/7/Onto-CMDB#PhysicalPosition
:PhysicalPosition rdf:type owl:DatatypeProperty ;
                  rdfs:subPropertyOf owl:topDataProperty ;
                  rdfs:domain :Location ;
                  rdfs:range xsd:string ;
                  rdfs:comment "Position is a free-form string that indicates the placement of a PhysicalElement. It can specify slot information on a HostingBoard, mounting site in a Cabinet, or latitude and longitude information, for example, from a GPS. It is part of the key of the Location object."^^xsd:string .


###  http://www.semanticweb.org/defaultuser/ontologies/2020/7/Onto-CMDB#PrimaryStatus
:PrimaryStatus rdf:type owl:DatatypeProperty ;
               rdfs:subPropertyOf owl:topDataProperty ;
               rdfs:domain :ManagedSystemElement ;
               rdfs:range rdf:PlainLiteral ;
               rdfs:comment "PrimaryStatus provides a high level status value, intended to align with Red-Yellow-Green type representation of status. PrimaryStatus consists of one of the following values: Unknown, OK, Degraded or Error. \"Unknown\" indicates the implementation is in general capable of returning this property, but is unable to do so at this time. \"OK\" indicates the ManagedElement is functioning normally. \"Degraded\" indicates the ManagedElement is functioning below normal. \"Error\" indicates the ManagedElement is in an Error condition."^^xsd:string .


###  http://www.semanticweb.org/defaultuser/ontologies/2020/7/Onto-CMDB#ProductTitle
:ProductTitle rdf:type owl:DatatypeProperty ;
              rdfs:subPropertyOf owl:topDataProperty ;
              rdfs:domain :SWID ;
              rdfs:range xsd:string ;
              rdfs:comment "Identifies the application. Accurately identifies the application. See ISO/IEC 19770-2:2009 for guidance."^^xsd:string .


###  http://www.semanticweb.org/defaultuser/ontologies/2020/7/Onto-CMDB#ReleaseDate
:ReleaseDate rdf:type owl:DatatypeProperty ;
             rdfs:subPropertyOf owl:topDataProperty ;
             rdfs:domain :SoftwareIdentity ;
             rdfs:range xsd:dateTime ;
             rdfs:comment "The date the software was released."^^xsd:string .


###  http://www.semanticweb.org/defaultuser/ontologies/2020/7/Onto-CMDB#RevisionLevel
:RevisionLevel rdf:type owl:DatatypeProperty ;
               rdfs:subPropertyOf owl:topDataProperty ;
               rdfs:domain :FRU ;
               rdfs:range xsd:string ;
               rdfs:comment "The FRU's revision level."^^xsd:string .


###  http://www.semanticweb.org/defaultuser/ontologies/2020/7/Onto-CMDB#RevisionNumber
:RevisionNumber rdf:type owl:DatatypeProperty ;
                rdfs:subPropertyOf owl:topDataProperty ;
                rdfs:domain :SoftwareIdentity ;
                rdfs:range xsd:integer ;
                rdfs:comment "The revision or maintenance release component of the software's version information - for example, '3' from version 12.1(3)T. This property is defined as a numeric value to allow the determination of 'newer' vs. 'older' releases. A 'newer' revision is indicated by a larger numeric value."^^xsd:string .


###  http://www.semanticweb.org/defaultuser/ontologies/2020/7/Onto-CMDB#SKU
:SKU rdf:type owl:DatatypeProperty ;
     rdfs:subPropertyOf owl:topDataProperty ;
     rdfs:domain :Product ;
     rdfs:range xsd:string ;
     rdfs:comment "The stock-keeping unit number."^^xsd:string .


###  http://www.semanticweb.org/defaultuser/ontologies/2020/7/Onto-CMDB#SerialNumber
:SerialNumber rdf:type owl:DatatypeProperty ;
              rdfs:subPropertyOf owl:topDataProperty ;
              rdfs:domain :ManagedSystemElement ;
              rdfs:range xsd:string ;
              rdfs:comment "A manufacturer-allocated number used to identify the Physical Element."^^xsd:string .


###  http://www.semanticweb.org/defaultuser/ontologies/2020/7/Onto-CMDB#ShortIdentifier
:ShortIdentifier rdf:type owl:DatatypeProperty ;
                 rdfs:subPropertyOf owl:topDataProperty ;
                 rdfs:domain :SPDX ;
                 rdfs:range xsd:string ;
                 rdfs:comment "A license identifier is a human readable short text string that uniquely identifies a license. For example: MIT"^^xsd:string .


###  http://www.semanticweb.org/defaultuser/ontologies/2020/7/Onto-CMDB#SoftwareCreator
:SoftwareCreator rdf:type owl:DatatypeProperty ;
                 rdfs:subPropertyOf owl:topDataProperty ;
                 rdfs:domain :SWID ;
                 rdfs:range xsd:string ;
                 rdfs:comment "Identifies the creator of the software.Identifies the application creator.See ISO/IEC 19770-2:2009 for guidance."^^xsd:string .


###  http://www.semanticweb.org/defaultuser/ontologies/2020/7/Onto-CMDB#SoftwareLicensor
:SoftwareLicensor rdf:type owl:DatatypeProperty ;
                  rdfs:subPropertyOf owl:topDataProperty ;
                  rdfs:domain :SWID ;
                  rdfs:range xsd:string ;
                  rdfs:comment "Identifies the licensor who owns the software copyright. See ISO/IEC 19770-2:2009 for guidance."^^xsd:string .


###  http://www.semanticweb.org/defaultuser/ontologies/2020/7/Onto-CMDB#Tag
:Tag rdf:type owl:DatatypeProperty ;
     rdfs:subPropertyOf owl:topDataProperty ;
     rdfs:domain :PhysicalElement ;
     rdfs:range rdf:PlainLiteral ;
     rdfs:comment "An arbitrary string that uniquely identifies the Physical Element and serves as the key of the Element. The Tag property can contain information such as asset tag or serial number data. The key for PhysicalElement is placed very high in the object hierarchy in order to independently identify the hardware or entity, regardless of physical placement in or on Cabinets, Adapters, and so on. For example, a hotswappable or removable component can be taken from its containing (scoping) package and be temporarily unused. The object still continues to exist and can even be inserted into a different scoping container. Therefore, the key for Physical Element is an arbitrary string and is defined independently of any placement or location-oriented hierarchy."^^xsd:string .


###  http://www.semanticweb.org/defaultuser/ontologies/2020/7/Onto-CMDB#TagCreator
:TagCreator rdf:type owl:DatatypeProperty ;
            rdfs:subPropertyOf owl:topDataProperty ;
            rdfs:domain :SWID ;
            rdfs:range xsd:string ;
            rdfs:comment """Identifies the tag creator.Identifies the tag creator. See ISO/IEC 19770-2:2009 for guidance.
Example data format:
“regid.2007-01.com.agnitioadvisors,BU-A”
where:
regid = registered id
2007-01 = the year and first month the domain was registered (yyyy-mm)
com = the upper level domain
AgnitioAdvisors = the domain name
BU-A = the sub-unit creating the SWID tag
xxx = the name of the business unit (BU) that created the SWID tag
Note that everything after the comma ‘,’ is optional and only required if a software title is specific to a particular business unite."""^^xsd:string .


###  http://www.semanticweb.org/defaultuser/ontologies/2020/7/Onto-CMDB#TargetOperatingSystems
:TargetOperatingSystems rdf:type owl:DatatypeProperty ;
                        rdfs:subPropertyOf owl:topDataProperty ;
                        rdfs:domain :SoftwareIdentity ;
                        rdfs:range xsd:string ;
                        rdfs:comment """Specifies the target operating systems of the software.

Unknown, Other, MACOS, ATTUNIX, DGUX, DECNT, Tru64 UNIX, OpenVMS, HPUX, AIX, MVS, OS400, OS/2, JavaVM, MSDOS, WIN3x, WIN95, WIN98, WINNT, WINCE, NCR3000, NetWare, OSF, DC/OS, Reliant UNIX, SCO UnixWare, SCO OpenServer, Sequent, IRIX, Solaris, SunOS, U6000, ASERIES, HP NonStop OS, HP NonStop OSS, BS2000, LINUX, Lynx, XENIX, VM, Interactive UNIX, BSDUNIX, FreeBSD, NetBSD, GNU Hurd, OS9, MACH Kernel, Inferno, QNX, EPOC, IxWorks, VxWorks, MiNT, BeOS, HP MPE, NextStep, PalmPilot, Rhapsody, Windows 2000, Dedicated, OS/390, VSE, TPF, Windows (R) Me, Caldera Open UNIX, OpenBSD, Not Applicable, Windows XP, z/OS, Microsoft Windows Server 2003, Microsoft Windows Server 2003 64-Bit, Windows XP 64-Bit, Windows XP Embedded, Windows Vista, Windows Vista 64-Bit, Windows Embedded for Point of Service, Microsoft Windows Server 2008, Microsoft Windows Server 2008 64-Bit, FreeBSD 64-Bit, RedHat Enterprise Linux, RedHat Enterprise Linux 64-Bit, Solaris 64-Bit, SUSE, SUSE 64-Bit, SLES, SLES 64-Bit, Novell OES, Novell Linux Desktop, Sun Java Desktop System, Mandriva, Mandriva 64-Bit, TurboLinux, TurboLinux 64-Bit, Ubuntu, Ubuntu 64-Bit, Debian, Debian 64-Bit, Linux 2.4.x, Linux 2.4.x 64-Bit, Linux 2.6.x, Linux 2.6.x 64-Bit, Linux 64-Bit, Other 64-Bit, Microsoft Windows Server 2008 R2, VMware ESXi, Microsoft Windows 7, CentOS 32-bit, CentOS 64-bit, Oracle Linux 32-bit, Oracle Linux 64-bit, eComStation 32-bitx, Microsoft Windows Server 2011, Microsoft Windows Server 2012, Microsoft Windows 8, Microsoft Windows 8 64-bit, Microsoft Windows Server 2012 R2, Microsoft Windows Server 2016, Microsoft Windows 8.1, Microsoft Windows 8.1 64-bit, Microsoft Windows 10, Microsoft Windows 10 64-bit"""^^xsd:string .


###  http://www.semanticweb.org/defaultuser/ontologies/2020/7/Onto-CMDB#Text
:Text rdf:type owl:DatatypeProperty ;
      rdfs:subPropertyOf owl:topDataProperty ;
      rdfs:domain :SPDX ;
      rdfs:range xsd:string ;
      rdfs:comment """For example: 

Copyright (c) <year> <copyright holders>

Permission is hereby granted, free of charge, to any person obtaining a copy of this software and associated documentation files (the \"Software\"), to deal in the Software without restriction, including without limitation the rights to use, copy, modify, merge, publish, distribute, sublicense, and/or sell copies of the Software, and to permit persons to whom the Software is furnished to do so, subject to the following conditions:

The above copyright notice and this permission notice (including the next paragraph) shall be included in all copies or substantial portions of the Software.

THE SOFTWARE IS PROVIDED \"AS IS\", WITHOUT WARRANTY OF ANY KIND, EXPRESS OR IMPLIED, INCLUDING BUT NOT LIMITED TO THE WARRANTIES OF MERCHANTABILITY, FITNESS FOR A PARTICULAR PURPOSE AND NONINFRINGEMENT. IN NO EVENT SHALL THE AUTHORS OR COPYRIGHT HOLDERS BE LIABLE FOR ANY CLAIM, DAMAGES OR OTHER LIABILITY, WHETHER IN AN ACTION OF CONTRACT, TORT OR OTHERWISE, ARISING FROM, OUT OF OR IN CONNECTION WITH THE SOFTWARE OR THE USE OR OTHER DEALINGS IN THE SOFTWARE."""^^xsd:string .


###  http://www.semanticweb.org/defaultuser/ontologies/2020/7/Onto-CMDB#UserTracking
:UserTracking rdf:type owl:DatatypeProperty ;
              rdfs:subPropertyOf owl:topDataProperty ;
              rdfs:domain :PhysicalElement ;
              rdfs:range xsd:string ;
              rdfs:comment "User-assigned and writeable asset-tracking identifier for the PhysicalElement."^^xsd:string .


###  http://www.semanticweb.org/defaultuser/ontologies/2020/7/Onto-CMDB#Vendor
:Vendor rdf:type owl:DatatypeProperty ;
        rdfs:subPropertyOf owl:topDataProperty ;
        rdfs:domain :FRU ;
        rdfs:range rdf:PlainLiteral ;
        rdfs:comment "The name of the FRU's supplier."^^xsd:string .


###  http://www.semanticweb.org/defaultuser/ontologies/2020/7/Onto-CMDB#VendorEquipmentType
:VendorEquipmentType rdf:type owl:DatatypeProperty ;
                     rdfs:subPropertyOf owl:topDataProperty ;
                     rdfs:domain :PhysicalElement ;
                     rdfs:range xsd:string ;
                     rdfs:comment "A vendor-specific hardware type for the PhysicalElement. It describes the specific equipment type for the element, as defined by the vendor or manufacturer."^^xsd:string .


###  http://www.semanticweb.org/defaultuser/ontologies/2020/7/Onto-CMDB#Version
:Version rdf:type owl:DatatypeProperty ;
         rdfs:subPropertyOf owl:topDataProperty ;
         rdfs:domain :PhysicalElement ;
         rdfs:range xsd:string ;
         rdfs:comment "A string that indicates the version of the PhysicalElement"^^xsd:string .


###  http://www.semanticweb.org/defaultuser/ontologies/2020/7/Onto-CMDB#VersionString
:VersionString rdf:type owl:DatatypeProperty ;
               rdfs:subPropertyOf owl:topDataProperty ;
               rdfs:domain :SoftwareIdentity ;
               rdfs:range xsd:string ;
               rdfs:comment "A string representing the complete software version information - for example, '12.1(3)T'. This string and the numeric major/minor/revision/build properties are complementary. Since vastly different representations and semantics exist for versions, it is not assumed that one representation is sufficient to permit a client to perform computations (i.e., the values are numeric) and a user to recognize the software's version (i.e., the values are understandable and readable). Hence, both numeric and string representations of version are provided."^^xsd:string .


###  http://www.semanticweb.org/defaultuser/ontologies/2020/7/Onto-CMDB#WarrantyDuration
:WarrantyDuration rdf:type owl:DatatypeProperty ;
                  rdfs:subPropertyOf owl:topDataProperty ;
                  rdfs:domain :Product ;
                  rdfs:range xsd:integer ;
                  rdfs:comment "If this Product is under warranty, the duration of the warranty in days."^^xsd:string .


###  http://www.semanticweb.org/defaultuser/ontologies/2020/7/Onto-CMDB#WarrantyStartDate
:WarrantyStartDate rdf:type owl:DatatypeProperty ;
                   rdfs:subPropertyOf owl:topDataProperty ;
                   rdfs:domain :Product ;
                   rdfs:range xsd:dateTime ;
                   rdfs:comment "If this Product is under warranty, the start date of the warranty."^^xsd:string .


###  http://www.semanticweb.org/defaultuser/ontologies/2020/7/Onto-CMDB#WebPages
:WebPages rdf:type owl:DatatypeProperty ;
          rdfs:subPropertyOf owl:topDataProperty ;
          rdfs:domain :SPDX ;
          rdfs:range xsd:string ;
          rdfs:comment "Other web pages for this license."^^xsd:string .


#################################################################
#    Classes
#################################################################

###  http://www.semanticweb.org/defaultuser/ontologies/2020/7/Onto-CMDB#FRU
:FRU rdf:type owl:Class ;
     rdfs:subClassOf :ManagedElement ;
     opla-sd:entityPosition [ opla-sd:entityPositionX "125.91659479562537"^^xsd:double ;
                              opla-sd:entityPositionY "45.88204538672695"^^xsd:double ;
                              rdfs:comment "This is an entity positioning annotation generated by CoModIDE (https://comodide.com/). Removing this annotation will break rendering the CoModIDE schema diagram view."@en
                            ] ;
     rdfs:comment "The FRU class is a vendor-defined collection of Products and/or PhysicalElements that is associated with a Product for the purpose of supporting, maintaining or upgrading that Product at the customer's location. FRU is an acronym for 'field replaceable unit'."^^xsd:string .


###  http://www.semanticweb.org/defaultuser/ontologies/2020/7/Onto-CMDB#Location
:Location rdf:type owl:Class ;
          rdfs:subClassOf :ManagedSystemElement .


###  http://www.semanticweb.org/defaultuser/ontologies/2020/7/Onto-CMDB#ManagedElement
:ManagedElement rdf:type owl:Class ;
                opla-sd:entityPosition [ opla-sd:entityPositionX "185.9162982628709"^^xsd:double ;
                                         opla-sd:entityPositionY "295.0637332535682"^^xsd:double ;
                                         rdfs:comment "This is an entity positioning annotation generated by CoModIDE (https://comodide.com/). Removing this annotation will break rendering the CoModIDE schema diagram view."@en
                                       ] ;
                rdfs:comment "ManagedElement is an abstract class that provides a common superclass."^^xsd:string .


###  http://www.semanticweb.org/defaultuser/ontologies/2020/7/Onto-CMDB#ManagedSystemElement
:ManagedSystemElement rdf:type owl:Class ;
                      rdfs:subClassOf :ManagedElement ;
                      owl:disjointWith :Product ;
                      opla-sd:entityPosition [ opla-sd:entityPositionX "360.1391270866579"^^xsd:double ;
                                               opla-sd:entityPositionY "400.1452533215478"^^xsd:double ;
                                               rdfs:comment "This is an entity positioning annotation generated by CoModIDE (https://comodide.com/). Removing this annotation will break rendering the CoModIDE schema diagram view."@en
                                             ] ;
                      rdfs:comment "Any distinguishable component of a System is a candidate for inclusion in this class. Examples of system components include: - software components such as application servers, databases, and applications - operating system components such as files, processes, and threads - device components such as disk drives, controllers, processors, and printers - physical components such as chips and cards."^^xsd:string .


###  http://www.semanticweb.org/defaultuser/ontologies/2020/7/Onto-CMDB#PhysicalElement
:PhysicalElement rdf:type owl:Class ;
                 rdfs:subClassOf :ManagedSystemElement ;
                 owl:disjointWith :SoftwareIdentity ;
                 opla-sd:entityPosition [ opla-sd:entityPositionX "509.96779175836207"^^xsd:double ;
                                          opla-sd:entityPositionY "129.97908426746073"^^xsd:double ;
                                          rdfs:comment "This is an entity positioning annotation generated by CoModIDE (https://comodide.com/). Removing this annotation will break rendering the CoModIDE schema diagram view."@en
                                        ] ;
                 rdfs:comment "Instances of this class can be defined as an object that can be seen or touched. All Processes, Files, and LogicalDevices are considered not to be Physical Elements. For example, it is not possible to touch the functionality of a 'modem.' You can touch only the card or package that implements the modem. The same card could also implement a LAN adapter. PhysicalElements are tangible ManagedSystemElements that have a physical manifestation of some sort. Note that the properties of PhysicalElement describe a hardware entity. Possible replacement (FRU) information is defined by FRU association. This definition allows a client to determine what hardware can be replaced (FRUed) and what 'spare' parts might be required by a customer or engineer doing the replacement."^^xsd:string .


###  http://www.semanticweb.org/defaultuser/ontologies/2020/7/Onto-CMDB#Product
:Product rdf:type owl:Class ;
         rdfs:subClassOf :ManagedElement ;
         opla-sd:entityPosition [ opla-sd:entityPositionX "125.6208428994094"^^xsd:double ;
                                  opla-sd:entityPositionY "37.8752209545502"^^xsd:double ;
                                  rdfs:comment "This is an entity positioning annotation generated by CoModIDE (https://comodide.com/). Removing this annotation will break rendering the CoModIDE schema diagram view."@en
                                ] ;
         rdfs:comment "Product is a concrete class that aggregates PhysicalElements, SoftwareIdentity and/or other Products, and is acquired as a unit. Acquisition implies an agreement between supplier and consumer which may have implications to Product licensing, support and warranty."^^xsd:string .


###  http://www.semanticweb.org/defaultuser/ontologies/2020/7/Onto-CMDB#SPDX
:SPDX rdf:type owl:Class ;
      rdfs:subClassOf :SoftwareIdentity ;
      opla-sd:entityPosition [ opla-sd:entityPositionX "85.16352403219078"^^xsd:double ;
                               opla-sd:entityPositionY "207.63296031451327"^^xsd:double ;
                               rdfs:comment "This is an entity positioning annotation generated by CoModIDE (https://comodide.com/). Removing this annotation will break rendering the CoModIDE schema diagram view."@en
                             ] ;
      rdfs:comment "The Software Package Data Exchange® (SPDX®) specification is a standard format for communicating the components, licenses and copyrights associated with a software package. The need to identify the license for open source software is critical for both reporting purposes and license compliance."^^xsd:string .


###  http://www.semanticweb.org/defaultuser/ontologies/2020/7/Onto-CMDB#SWID
:SWID rdf:type owl:Class ;
      rdfs:subClassOf :SoftwareIdentity ;
      opla-sd:entityPosition [ opla-sd:entityPositionX "119.58813663955416"^^xsd:double ;
                               opla-sd:entityPositionY "55.419672363863306"^^xsd:double ;
                               rdfs:comment "This is an entity positioning annotation generated by CoModIDE (https://comodide.com/). Removing this annotation will break rendering the CoModIDE schema diagram view."@en
                             ] ;
      rdfs:comment "According to ISO/IEC 19770-2:2009  the SWID tag is an XML file containing authoritative identification and management information about a software product. Accurate identification of software allows organizations to support internal requirements and comply with regulatory requirements."^^xsd:string .


###  http://www.semanticweb.org/defaultuser/ontologies/2020/7/Onto-CMDB#SoftwareIdentity
:SoftwareIdentity rdf:type owl:Class ;
                  rdfs:subClassOf :ManagedSystemElement ;
                  opla-sd:entityPosition [ opla-sd:entityPositionX "42.72389493352092"^^xsd:double ;
                                           opla-sd:entityPositionY "144.5071153139528"^^xsd:double ;
                                           rdfs:comment "This is an entity positioning annotation generated by CoModIDE (https://comodide.com/). Removing this annotation will break rendering the CoModIDE schema diagram view."@en
                                         ] ;
                  rdfs:comment "SoftwareIdentity provides descriptive information about a software component for asset tracking and/or installation dependency management"^^xsd:string .


#################################################################
#    Individuals
#################################################################

###  http://www.semanticweb.org/defaultuser/ontologies/2020/7/Onto-CMDB#CISCO1841_001
:CISCO1841_001 rdf:type owl:NamedIndividual ,
                        :ManagedSystemElement ;
               :hasLocation :M1_Riihimaki ;
               :hasPhysicalElement :Cisco_1841_chassis ,
                                   <http://www.semanticweb.org/defaultuser/ontologies/2020/7/Onto-CMDB#4-port_10/100BASE-T_Ethernet_switch_HWIC> ;
               :hasSoftwareIdentity :CISCO_IOS_12_4 ;
               :InstallDate "2020-07-26T21:32:52"^^xsd:dateTime ;
               :PrimaryStatus "OK" ;
               :SerialNumber "FCZ122293NR"^^xsd:string .


###  http://www.semanticweb.org/defaultuser/ontologies/2020/7/Onto-CMDB#CISCO1841_002
:CISCO1841_002 rdf:type owl:NamedIndividual ,
                        :ManagedSystemElement ;
               :hasFRU :MEM1800-64CF ;
               :hasLocation :M1_Riihimaki ;
               :hasPhysicalElement :Cisco_1841_chassis ;
               :hasSoftwareIdentity :CISCO_IOS_15_0 ;
               :InstallDate "2020-07-26T21:32:52"^^xsd:dateTime ;
               :PrimaryStatus "OK" ;
               :SerialNumber "FCZ122294NR"^^xsd:string .


###  http://www.semanticweb.org/defaultuser/ontologies/2020/7/Onto-CMDB#CISCO1841_003
:CISCO1841_003 rdf:type owl:NamedIndividual ,
                        :ManagedSystemElement ;
               :hasLocation :M2_Riihimaki ;
               :hasManagedSystemElement :Cisco_1841_chassis ,
                                        <http://www.semanticweb.org/defaultuser/ontologies/2020/7/Onto-CMDB#4-port_G.SHDSL_WIC> ,
                                        <http://www.semanticweb.org/defaultuser/ontologies/2020/7/Onto-CMDB#4-port_10/100BASE-T_Ethernet_switch_HWIC> ;
               :hasSoftwareIdentity :CISCO_IOS_15_0 ;
               :InstallDate "2020-07-26T21:32:52"^^xsd:dateTime ;
               :PrimaryStatus "OK" ;
               :SerialNumber "FCZ122295NR"^^xsd:string .


###  http://www.semanticweb.org/defaultuser/ontologies/2020/7/Onto-CMDB#CISCO3750_001
:CISCO3750_001 rdf:type owl:NamedIndividual ,
                        :ManagedSystemElement ;
               :hasLocation :M2_Riihimaki ;
               :hasPhysicalElement <http://www.semanticweb.org/defaultuser/ontologies/2020/7/Onto-CMDB#Catalyst_3750_48_10/100> ;
               :hasSoftwareIdentity :CISCO_IOS_12_4 ;
               :InstallDate "2020-07-26T21:32:52"^^xsd:dateTime ;
               :PrimaryStatus "OK" ;
               :SerialNumber "FCZ122296NR"^^xsd:string .


###  http://www.semanticweb.org/defaultuser/ontologies/2020/7/Onto-CMDB#CISCO3750_002
:CISCO3750_002 rdf:type owl:NamedIndividual ,
                        :ManagedSystemElement ;
               :hasLocation :M2_Riihimaki ;
               :hasPhysicalElement <http://www.semanticweb.org/defaultuser/ontologies/2020/7/Onto-CMDB#Catalyst_3750_48_10/100> ;
               :hasSoftwareIdentity :CISCO_IOS_15_0 ;
               :InstallDate "2020-07-26T21:32:52"^^xsd:dateTime ;
               :PrimaryStatus "OK" ;
               :SerialNumber "FCZ122297NR"^^xsd:string .


###  http://www.semanticweb.org/defaultuser/ontologies/2020/7/Onto-CMDB#CISCO_1841
:CISCO_1841 rdf:type owl:NamedIndividual ,
                     :ManagedElement ;
            :hasFRU :MEM1800-64CF ;
            :hasManagedSystemElement :CISCO1841_001 ,
                                     :CISCO1841_002 ,
                                     :CISCO1841_003 ;
            :Caption "Cisco 1841"^^xsd:string ;
            :Description "Cisco 1841 Router"^^xsd:string ;
            :ElementName "Cisco 1841 Router"^^xsd:string ;
            :Generation "1"^^xsd:string ;
            :Name "Router"^^xsd:string .


###  http://www.semanticweb.org/defaultuser/ontologies/2020/7/Onto-CMDB#CISCO_CATALYST_3750
:CISCO_CATALYST_3750 rdf:type owl:NamedIndividual ,
                              :ManagedElement ;
                     :hasManagedSystemElement :CISCO3750_001 ,
                                              :CISCO3750_002 ;
                     :Caption "Cisco Catalyst 3750"^^xsd:string ;
                     :Description "Catalyst 3750V2-48PS Switch"^^xsd:string ;
                     :ElementName "Cisco Catalyst 3750V2-48PS Switch"^^xsd:string ;
                     :Generation "1"^^xsd:string ;
                     :Name "Switch"^^xsd:string .


###  http://www.semanticweb.org/defaultuser/ontologies/2020/7/Onto-CMDB#CISCO_IOS_12_4
:CISCO_IOS_12_4 rdf:type owl:NamedIndividual ,
                         :SoftwareIdentity ;
                :hasSPDX :IOS_BSD-3 ;
                :hasSWID :Cisco_IOS ;
                :ExtendedResourceType "zip"^^xsd:string ;
                :LargeBuildNumber 12 ;
                :MajorVersion 12 ;
                :MinorVersion 4 ;
                :ReleaseDate "2015-10-26T19:32:52+00:00"^^xsd:dateTime ;
                :RevisionNumber 1 ;
                :TargetOperatingSystems "IOS"^^xsd:string ;
                :VersionString "12.4(1)S"^^xsd:string ;
                rdfs:label "CISCO IOS"@fi .


###  http://www.semanticweb.org/defaultuser/ontologies/2020/7/Onto-CMDB#CISCO_IOS_15_0
:CISCO_IOS_15_0 rdf:type owl:NamedIndividual ,
                         :SoftwareIdentity ;
                :hasSPDX :IOS_BSD-3 ;
                :hasSWID :Cisco_IOS ;
                :ExtendedResourceType "zip"^^xsd:string ;
                :LargeBuildNumber 15 ;
                :MajorVersion 0 ,
                              15 ;
                :ReleaseDate "2017-10-26T19:32:52+00:00"^^xsd:dateTime ;
                :RevisionNumber 1 ;
                :TargetOperatingSystems "IOS"^^xsd:string ;
                :VersionString "15.0(1)S"^^xsd:string ;
                rdfs:label "CISCO IOS"@fi .


###  http://www.semanticweb.org/defaultuser/ontologies/2020/7/Onto-CMDB#Cisco1800
:Cisco1800 rdf:type owl:NamedIndividual ,
                    :Product ;
           :SKU "IPM7W00CRA"^^xsd:string ;
           :WarrantyDuration 600 ;
           :WarrantyStartDate "2015-10-26T19:32:52+00:00"^^xsd:dateTime .


###  http://www.semanticweb.org/defaultuser/ontologies/2020/7/Onto-CMDB#Cisco3750
:Cisco3750 rdf:type owl:NamedIndividual ,
                    :Product ;
           :SKU "IPM7W33CRA"^^xsd:string ;
           :WarrantyDuration 800 ;
           :WarrantyStartDate "2012-09-13T14:12:00+00:00"^^xsd:dateTime .


###  http://www.semanticweb.org/defaultuser/ontologies/2020/7/Onto-CMDB#Cisco_1841_chassis
:Cisco_1841_chassis rdf:type owl:NamedIndividual ,
                             :PhysicalElement ;
                    :ManufactureDate "2007-10-26T19:32:52+00:00"^^xsd:dateTime ;
                    :Manufacturer "Cisco"^^xsd:string ;
                    :Model "Router"^^xsd:string ;
                    :OtherIdentifyingInfo "27568452"^^xsd:string ;
                    :PartNumber "73-8191-66"^^xsd:string ;
                    :Tag "FOC10466XVR"^^xsd:string ;
                    :UserTracking "Z79263"^^xsd:string ;
                    :VendorEquipmentType "Router"^^xsd:string ;
                    :Version "4.0"^^xsd:string ,
                             "V1"^^xsd:string .


###  http://www.semanticweb.org/defaultuser/ontologies/2020/7/Onto-CMDB#Cisco_IOS
:Cisco_IOS rdf:type owl:NamedIndividual ,
                    :SWID ;
           :EntitlementRequiredIndicator "false"^^xsd:boolean ;
           :ProductTitle "Cisco IOS"^^xsd:string ;
           :SoftwareCreator "Cisco Inc."^^xsd:string ;
           :TagCreator "Cisco Inc."^^xsd:string .


###  http://www.semanticweb.org/defaultuser/ontologies/2020/7/Onto-CMDB#HPProliantDL380G6
:HPProliantDL380G6 rdf:type owl:NamedIndividual ,
                            :Product ;
                   :SKU "IPM7W23CRA"^^xsd:string ;
                   :WarrantyDuration 760 ;
                   :WarrantyStartDate "2016-01-02T13:22:00+00:00"^^xsd:dateTime .


###  http://www.semanticweb.org/defaultuser/ontologies/2020/7/Onto-CMDB#IOS_BSD-3
:IOS_BSD-3 rdf:type owl:NamedIndividual ,
                    :SPDX ;
           :FullName "BSD-3-Clause"^^xsd:string ;
           :Notes "The DPDK uses the Open Source BSD-3-Clause license for the core libraries and drivers."^^xsd:string ;
           :Text """Redistribution and use in source and binary forms, with or without modification, are permitted provided that the following conditions are met:

1. Redistributions of source code must retain the above copyright notice, this list of conditions and the following disclaimer.

2. Redistributions in binary form must reproduce the above copyright notice, this list of conditions and the following disclaimer in the documentation and/or other materials provided with the distribution.

3. Neither the name of the copyright holder nor the names of its contributors may be used to endorse or promote products derived from this software without specific prior written permission.

THIS SOFTWARE IS PROVIDED BY THE COPYRIGHT HOLDERS AND CONTRIBUTORS \"AS IS\" AND ANY EXPRESS OR IMPLIED WARRANTIES, INCLUDING, BUT NOT LIMITED TO, THE IMPLIED WARRANTIES OF MERCHANTABILITY AND FITNESS FOR A PARTICULAR PURPOSE ARE DISCLAIMED. IN NO EVENT SHALL THE COPYRIGHT HOLDER OR CONTRIBUTORS BE LIABLE FOR ANY DIRECT, INDIRECT, INCIDENTAL, SPECIAL, EXEMPLARY, OR CONSEQUENTIAL DAMAGES (INCLUDING, BUT NOT LIMITED TO, PROCUREMENT OF SUBSTITUTE GOODS OR SERVICES; LOSS OF USE, DATA, OR PROFITS; OR BUSINESS INTERRUPTION) HOWEVER CAUSED AND ON ANY THEORY OF LIABILITY, WHETHER IN CONTRACT, STRICT LIABILITY, OR TORT (INCLUDING NEGLIGENCE OR OTHERWISE) ARISING IN ANY WAY OUT OF THE USE OF THIS SOFTWARE, EVEN IF ADVISED OF THE POSSIBILITY OF SUCH DAMAGE."""^^xsd:string ;
           :WebPages "https://opensource.org/licenses/BSD-3-Clause"^^xsd:string .


###  http://www.semanticweb.org/defaultuser/ontologies/2020/7/Onto-CMDB#M1_Riihimaki
:M1_Riihimaki rdf:type owl:NamedIndividual ,
                       :Location ;
              :Address "Karjaportintie" ;
              :PhysicalPosition "HY4"^^xsd:string .


###  http://www.semanticweb.org/defaultuser/ontologies/2020/7/Onto-CMDB#M2_Riihimaki
:M2_Riihimaki rdf:type owl:NamedIndividual ,
                       :Location ;
              :Address "Karjaportintie" ;
              :PhysicalPosition "HY5"^^xsd:string .


###  http://www.semanticweb.org/defaultuser/ontologies/2020/7/Onto-CMDB#MEM1800-128CF
:MEM1800-128CF rdf:type owl:NamedIndividual ,
                        :FRU .


###  http://www.semanticweb.org/defaultuser/ontologies/2020/7/Onto-CMDB#MEM1800-64CF
:MEM1800-64CF rdf:type owl:NamedIndividual ,
                       :FRU .


###  http://www.semanticweb.org/defaultuser/ontologies/2020/7/Onto-CMDB#4-port_G.SHDSL_WIC
<http://www.semanticweb.org/defaultuser/ontologies/2020/7/Onto-CMDB#4-port_G.SHDSL_WIC> rdf:type owl:NamedIndividual ,
                                                                                                 :PhysicalElement ;
                                                                                        :ManufactureDate "2011-10-26T19:32:52+00:00"^^xsd:dateTime ;
                                                                                        :Manufacturer "Cisco"^^xsd:string ;
                                                                                        :Model "Interface card"^^xsd:string ;
                                                                                        :OtherIdentifyingInfo "34567845"^^xsd:string ;
                                                                                        :PartNumber "73-8191-11"^^xsd:string ;
                                                                                        :Tag "FOC10481XVR"^^xsd:string ;
                                                                                        :UserTracking "Z30673"^^xsd:string ;
                                                                                        :VendorEquipmentType "One port G.shdsl WIC with 4-wire support"^^xsd:string ;
                                                                                        :Version "5.0"^^xsd:string ,
                                                                                                 "V3" .


###  http://www.semanticweb.org/defaultuser/ontologies/2020/7/Onto-CMDB#4-port_10/100BASE-T_Ethernet_switch_HWIC
<http://www.semanticweb.org/defaultuser/ontologies/2020/7/Onto-CMDB#4-port_10/100BASE-T_Ethernet_switch_HWIC> rdf:type owl:NamedIndividual ,
                                                                                                                       :PhysicalElement ;
                                                                                                              :ManufactureDate "2001-10-26T19:32:52+00:00"^^xsd:dateTime ;
                                                                                                              :Manufacturer "Cisco"^^xsd:string ;
                                                                                                              :Model "Interface card"^^xsd:string ;
                                                                                                              :OtherIdentifyingInfo "24234423"^^xsd:string ;
                                                                                                              :PartNumber "73-8191-06"^^xsd:string ;
                                                                                                              :Tag "FOC10485XVR"^^xsd:string ;
                                                                                                              :UserTracking "Z43876"^^xsd:string ;
                                                                                                              :VendorEquipmentType "Ethernet switch interface card"^^xsd:string ;
                                                                                                              :Version "4.0"^^xsd:string ,
                                                                                                                       "V2" .


###  http://www.semanticweb.org/defaultuser/ontologies/2020/7/Onto-CMDB#Catalyst_3750_48_10/100
<http://www.semanticweb.org/defaultuser/ontologies/2020/7/Onto-CMDB#Catalyst_3750_48_10/100> rdf:type owl:NamedIndividual ,
                                                                                                      :PhysicalElement ;
                                                                                             :ManufactureDate "2011-10-26T19:32:52+00:00"^^xsd:dateTime ;
                                                                                             :Manufacturer "Cisco"^^xsd:string ;
                                                                                             :Model "Switch"^^xsd:string ;
                                                                                             :OtherIdentifyingInfo "849776543"^^xsd:string ;
                                                                                             :PartNumber "73-8191-22"^^xsd:string ;
                                                                                             :Tag "FOC10455XVR"^^xsd:string ;
                                                                                             :UserTracking "Z22865"^^xsd:string ;
                                                                                             :VendorEquipmentType "Switch"^^xsd:string ;
                                                                                             :Version "6.0"^^xsd:string ,
                                                                                                      "V!"^^xsd:string .


[ ontodebug:axiom "hasFRU Range FRU"^^xsd:string ;
  ontodebug:type "true"^^xsd:boolean
] .

[ ontodebug:axiom "hasName Domain ManagedSystemElement"^^xsd:string ;
   ontodebug:type "true"^^xsd:boolean
 ] .

[ ontodebug:axiom "WarrantyDuration Domain SoftwareIdentity"^^xsd:string ;
   ontodebug:type "false"^^xsd:boolean
 ] .

[ ontodebug:axiom "OperatingStatus DisjointWith SoftwareIdentity"^^xsd:string ;
   ontodebug:type "true"^^xsd:boolean
 ] .

[ ontodebug:axiom "OperatingStatus Domain PhysicalElement"^^xsd:string ;
   ontodebug:type "true"^^xsd:boolean
 ] .

[ ontodebug:axiom "Manufacturer Domain ManagedElement"^^xsd:string ;
   ontodebug:type "true"^^xsd:boolean
 ] .

[ ontodebug:axiom "CISCO_CATALYST_3750 Caption \"Cisco Catalyst 3750\"^^string"^^xsd:string ;
   ontodebug:type "true"^^xsd:boolean
 ] .

[ ontodebug:axiom "Classifications DisjointWith OperatingStatus"^^xsd:string ;
   ontodebug:type "true"^^xsd:boolean
 ] .

[ ontodebug:axiom "SPDX SubClassOf ManagedSystemElement"^^xsd:string ;
   ontodebug:type "true"^^xsd:boolean
 ] .

[ ontodebug:axiom "SoftwareCreator Domain PhysicalElement"^^xsd:string ;
   ontodebug:type "false"^^xsd:boolean
 ] .

[ ontodebug:axiom "FRU SubClassOf ManagedSystemElement"^^xsd:string ;
   ontodebug:type "false"^^xsd:boolean
 ] .

[ ontodebug:axiom "SerialNumber Domain PhysicalElement"^^xsd:string ;
   ontodebug:type "true"^^xsd:boolean
 ] .

[ ontodebug:axiom "SPDX EquivalentTo SWID"^^xsd:string ;
   ontodebug:type "false"^^xsd:boolean
 ] .

[ ontodebug:axiom "Manufacturer Domain SoftwareIdentity"^^xsd:string ;
   ontodebug:type "false"^^xsd:boolean
 ] .

[ ontodebug:axiom "Name Domain ManagedElement"^^xsd:string ;
   ontodebug:type "true"^^xsd:boolean
 ] .

[ ontodebug:axiom "Unknown Type Classifications"^^xsd:string ;
   ontodebug:type "true"^^xsd:boolean
 ] .

[ ontodebug:axiom "Family Domain FRU"^^xsd:string ;
   ontodebug:type "false"^^xsd:boolean
 ] .

[ ontodebug:axiom "hasName Domain ManagedElement"^^xsd:string ;
   ontodebug:type "true"^^xsd:boolean
 ] .

[ ontodebug:axiom "Classifications SubClassOf Product"^^xsd:string ;
   ontodebug:type "false"^^xsd:boolean
 ] .

[ ontodebug:axiom "hasLocation Range SoftwareIdentity"^^xsd:string ;
   ontodebug:type "false"^^xsd:boolean
 ] .

[ ontodebug:axiom "WarrantyDuration Domain SPDX"^^xsd:string ;
   ontodebug:type "false"^^xsd:boolean
 ] .

[ ontodebug:axiom "hasProduct Range ManagedElement"^^xsd:string ;
   ontodebug:type "true"^^xsd:boolean
 ] .

[ ontodebug:axiom "Name Domain PhysicalElement"^^xsd:string ;
   ontodebug:type "true"^^xsd:boolean
 ] .

[ ontodebug:axiom "hasProduct Range SoftwareIdentity"^^xsd:string ;
   ontodebug:type "true"^^xsd:boolean
 ] .

[ ontodebug:axiom "Location DisjointWith ManagedSystemElement"^^xsd:string ;
   ontodebug:type "true"^^xsd:boolean
 ] .

[ ontodebug:axiom "Classifications SubClassOf Product"^^xsd:string ;
   ontodebug:type "false"^^xsd:boolean
 ] .

[ ontodebug:axiom "FRU DisjointWith ManagedSystemElement"^^xsd:string ;
   ontodebug:type "true"^^xsd:boolean
 ] .

[ ontodebug:axiom "Manufacturer Domain ManagedElement"^^xsd:string ;
   ontodebug:type "true"^^xsd:boolean
 ] .

[ ontodebug:axiom "hasName Domain ManagedSystemElement"^^xsd:string ;
   ontodebug:type "true"^^xsd:boolean
 ] .

[ ontodebug:axiom "Caption Domain Location"^^xsd:string ;
   ontodebug:type "true"^^xsd:boolean
 ] .

[ ontodebug:axiom "hasProduct Range SoftwareIdentity"^^xsd:string ;
   ontodebug:type "true"^^xsd:boolean
 ] .

[ ontodebug:axiom "hasName Domain ManagedSystemElement"^^xsd:string ;
   ontodebug:type "true"^^xsd:boolean
 ] .

[ ontodebug:axiom "hasProduct Range ManagedElement"^^xsd:string ;
   ontodebug:type "true"^^xsd:boolean
 ] .

[ ontodebug:axiom "hasLocation Range SoftwareIdentity"^^xsd:string ;
   ontodebug:type "false"^^xsd:boolean
 ] .

[ ontodebug:axiom "OperatingStatus DisjointWith SoftwareIdentity"^^xsd:string ;
   ontodebug:type "true"^^xsd:boolean
 ] .

[ ontodebug:axiom "OperatingStatus Domain PhysicalElement"^^xsd:string ;
   ontodebug:type "true"^^xsd:boolean
 ] .

[ ontodebug:axiom "Location SubClassOf ManagedSystemElement"^^xsd:string ;
   ontodebug:type "false"^^xsd:boolean
 ] .

[ ontodebug:axiom "Caption Domain Location"^^xsd:string ;
   ontodebug:type "true"^^xsd:boolean
 ] .

[ ontodebug:axiom "Classifications DisjointWith OperatingStatus"^^xsd:string ;
   ontodebug:type "true"^^xsd:boolean
 ] .

[ ontodebug:axiom "SPDX EquivalentTo SWID"^^xsd:string ;
   ontodebug:type "false"^^xsd:boolean
 ] .

[ ontodebug:axiom "hasName Domain ManagedElement"^^xsd:string ;
   ontodebug:type "true"^^xsd:boolean
 ] .

[ ontodebug:axiom "Manufacturer Domain SoftwareIdentity"^^xsd:string ;
   ontodebug:type "false"^^xsd:boolean
 ] .

[ ontodebug:axiom "OperatingStatus DisjointWith SoftwareIdentity"^^xsd:string ;
   ontodebug:type "true"^^xsd:boolean
 ] .

[ ontodebug:axiom "Classifications DisjointWith OperatingStatus"^^xsd:string ;
   ontodebug:type "true"^^xsd:boolean
 ] .

[ ontodebug:axiom "FRU and Product SubClassOf ManagedElement"^^xsd:string ;
   ontodebug:type "true"^^xsd:boolean
 ] .

[ ontodebug:axiom "Classifications DisjointWith OperatingStatus"^^xsd:string ;
   ontodebug:type "true"^^xsd:boolean
 ] .

[ ontodebug:axiom "ManagedSystemElement DisjointWith Product"^^xsd:string ;
   ontodebug:type "true"^^xsd:boolean
 ] .

[ ontodebug:axiom "hasProduct Range SoftwareIdentity"^^xsd:string ;
   ontodebug:type "true"^^xsd:boolean
 ] .

[ ontodebug:axiom "hasProduct Range FRU"^^xsd:string ;
   ontodebug:type "true"^^xsd:boolean
 ] .

[ ontodebug:axiom "SPDX EquivalentTo SWID"^^xsd:string ;
   ontodebug:type "false"^^xsd:boolean
 ] .

[ ontodebug:axiom "hasName Domain ManagedSystemElement"^^xsd:string ;
   ontodebug:type "true"^^xsd:boolean
 ] .

[ ontodebug:axiom "Manufacturer Domain ManagedElement"^^xsd:string ;
   ontodebug:type "true"^^xsd:boolean
 ] .

[ ontodebug:axiom "hasName Domain ManagedElement"^^xsd:string ;
   ontodebug:type "true"^^xsd:boolean
 ] .

[ ontodebug:axiom "Unknown Type Classifications"^^xsd:string ;
   ontodebug:type "true"^^xsd:boolean
 ] .

[ ontodebug:axiom "Location DisjointWith ManagedSystemElement"^^xsd:string ;
   ontodebug:type "true"^^xsd:boolean
 ] .

[ ontodebug:axiom "Caption Domain FRU"^^xsd:string ;
   ontodebug:type "true"^^xsd:boolean
 ] .

[ ontodebug:axiom "Manufacturer Domain ManagedElement"^^xsd:string ;
   ontodebug:type "true"^^xsd:boolean
 ] .

[ ontodebug:axiom "Product SubClassOf ManagedSystemElement"^^xsd:string ;
   ontodebug:type "false"^^xsd:boolean
 ] .

[ ontodebug:axiom "ManagedSystemElement DisjointWith Product"^^xsd:string ;
   ontodebug:type "true"^^xsd:boolean
 ] .

[ ontodebug:axiom "hasFRU Range FRU"^^xsd:string ;
   ontodebug:type "true"^^xsd:boolean
 ] .

[ ontodebug:axiom "Manufacturer Domain ManagedElement"^^xsd:string ;
   ontodebug:type "true"^^xsd:boolean
 ] .

[ ontodebug:axiom "hasName Domain ManagedElement"^^xsd:string ;
   ontodebug:type "true"^^xsd:boolean
 ] .

[ ontodebug:axiom "hasName Domain ManagedElement"^^xsd:string ;
   ontodebug:type "true"^^xsd:boolean
 ] .

[ ontodebug:axiom "hasName Domain ManagedElement"^^xsd:string ;
   ontodebug:type "true"^^xsd:boolean
 ] .

[ ontodebug:axiom "hasProduct Range SPDX"^^xsd:string ;
   ontodebug:type "true"^^xsd:boolean
 ] .

[ ontodebug:axiom "ManagedSystemElement DisjointWith Product"^^xsd:string ;
   ontodebug:type "true"^^xsd:boolean
 ] .

[ ontodebug:axiom "hasName Domain ManagedElement"^^xsd:string ;
   ontodebug:type "true"^^xsd:boolean
 ] .

[ ontodebug:axiom "hasProduct Range ManagedSystemElement"^^xsd:string ;
   ontodebug:type "true"^^xsd:boolean
 ] .

[ ontodebug:axiom "Unknown Type Classifications"^^xsd:string ;
   ontodebug:type "true"^^xsd:boolean
 ] .

[ ontodebug:axiom "Caption Domain FRU"^^xsd:string ;
   ontodebug:type "true"^^xsd:boolean
 ] .

[ ontodebug:axiom "hasFRU Range FRU"^^xsd:string ;
   ontodebug:type "true"^^xsd:boolean
 ] .

[ ontodebug:axiom "Location DisjointWith ManagedSystemElement"^^xsd:string ;
   ontodebug:type "true"^^xsd:boolean
 ] .

[ ontodebug:axiom "Family Domain FRU"^^xsd:string ;
   ontodebug:type "false"^^xsd:boolean
 ] .

[ ontodebug:axiom "hasFRU Domain Product"^^xsd:string ;
   ontodebug:type "false"^^xsd:boolean
 ] .

[ ontodebug:axiom "Family Domain FRU"^^xsd:string ;
   ontodebug:type "false"^^xsd:boolean
 ] .

[ ontodebug:axiom "Classifications SubClassOf Product"^^xsd:string ;
   ontodebug:type "false"^^xsd:boolean
 ] .

[ ontodebug:axiom "FRU DisjointWith ManagedSystemElement"^^xsd:string ;
   ontodebug:type "true"^^xsd:boolean
 ] .

[ ontodebug:axiom "ManagedSystemElement DisjointWith Product"^^xsd:string ;
   ontodebug:type "true"^^xsd:boolean
 ] .

[ ontodebug:axiom "Location SubClassOf ManagedSystemElement"^^xsd:string ;
   ontodebug:type "false"^^xsd:boolean
 ] .

[ ontodebug:axiom "Location SubClassOf ManagedSystemElement"^^xsd:string ;
   ontodebug:type "false"^^xsd:boolean
 ] .

[ ontodebug:axiom "FRU and Product SubClassOf ManagedElement"^^xsd:string ;
   ontodebug:type "true"^^xsd:boolean
 ] .

[ ontodebug:axiom "Location DisjointWith ManagedSystemElement"^^xsd:string ;
   ontodebug:type "true"^^xsd:boolean
 ] .

[ ontodebug:axiom "hasName Domain ManagedSystemElement"^^xsd:string ;
   ontodebug:type "true"^^xsd:boolean
 ] .

[ ontodebug:axiom "hasName Domain ManagedElement"^^xsd:string ;
   ontodebug:type "true"^^xsd:boolean
 ] .

[ ontodebug:axiom "SPDX SubClassOf ManagedSystemElement"^^xsd:string ;
   ontodebug:type "true"^^xsd:boolean
 ] .

[ ontodebug:axiom "hasName Domain ManagedSystemElement"^^xsd:string ;
   ontodebug:type "true"^^xsd:boolean
 ] .

[ ontodebug:axiom "Family Domain FRU"^^xsd:string ;
   ontodebug:type "false"^^xsd:boolean
 ] .

[ ontodebug:axiom "hasFRU Domain Product"^^xsd:string ;
   ontodebug:type "false"^^xsd:boolean
 ] .

[ ontodebug:axiom "ManagedSystemElement DisjointWith Product"^^xsd:string ;
   ontodebug:type "true"^^xsd:boolean
 ] .

[ ontodebug:axiom "Name Domain ManagedElement"^^xsd:string ;
   ontodebug:type "true"^^xsd:boolean
 ] .

[ ontodebug:axiom "hasFRU Domain Product"^^xsd:string ;
   ontodebug:type "false"^^xsd:boolean
 ] .

[ ontodebug:axiom "FRU and Product SubClassOf ManagedElement"^^xsd:string ;
   ontodebug:type "true"^^xsd:boolean
 ] .

[ ontodebug:axiom "hasName Domain ManagedSystemElement"^^xsd:string ;
   ontodebug:type "true"^^xsd:boolean
 ] .

[ ontodebug:axiom "WarrantyDuration Domain SoftwareIdentity"^^xsd:string ;
   ontodebug:type "false"^^xsd:boolean
 ] .

[ ontodebug:axiom "hasName Domain ManagedSystemElement"^^xsd:string ;
   ontodebug:type "true"^^xsd:boolean
 ] .

[ ontodebug:axiom "Location SubClassOf ManagedSystemElement"^^xsd:string ;
   ontodebug:type "false"^^xsd:boolean
 ] .

[ ontodebug:axiom "FRU DisjointWith SPDX"^^xsd:string ;
   ontodebug:type "true"^^xsd:boolean
 ] .

[ ontodebug:axiom "hasName Domain ManagedSystemElement"^^xsd:string ;
   ontodebug:type "true"^^xsd:boolean
 ] .

[ ontodebug:axiom "Location DisjointWith ManagedSystemElement"^^xsd:string ;
   ontodebug:type "true"^^xsd:boolean
 ] .

[ ontodebug:axiom "FRU SubClassOf ManagedSystemElement"^^xsd:string ;
   ontodebug:type "false"^^xsd:boolean
 ] .

[ ontodebug:axiom "hasProduct Range PhysicalElement"^^xsd:string ;
   ontodebug:type "true"^^xsd:boolean
 ] .

[ ontodebug:axiom "Classifications DisjointWith OperatingStatus"^^xsd:string ;
   ontodebug:type "true"^^xsd:boolean
 ] .

[ ontodebug:axiom "FRU DisjointWith SPDX"^^xsd:string ;
   ontodebug:type "true"^^xsd:boolean
 ] .

[ ontodebug:axiom "hasName Domain ManagedSystemElement"^^xsd:string ;
   ontodebug:type "true"^^xsd:boolean
 ] .

[ ontodebug:axiom "Manufacturer Domain SoftwareIdentity"^^xsd:string ;
   ontodebug:type "false"^^xsd:boolean
 ] .

[ ontodebug:axiom "hasFRU Domain Product"^^xsd:string ;
   ontodebug:type "false"^^xsd:boolean
 ] .

[ ontodebug:axiom "hasName Domain ManagedElement"^^xsd:string ;
   ontodebug:type "true"^^xsd:boolean
 ] .

[ ontodebug:axiom "hasFRU Range FRU"^^xsd:string ;
   ontodebug:type "true"^^xsd:boolean
 ] .

[ ontodebug:axiom "WarrantyDuration Domain SPDX"^^xsd:string ;
   ontodebug:type "false"^^xsd:boolean
 ] .

[ opla-sd:entityPositionX "215.7828295953237"^^xsd:double ;
   opla-sd:entityPositionY "76.50558656596547"^^xsd:double ;
   rdfs:comment "This is an entity positioning annotation generated by CoModIDE (https://comodide.com/). Removing this annotation will break rendering the CoModIDE schema diagram view."@en
 ] .

[ ontodebug:axiom "SPDX EquivalentTo SWID"^^xsd:string ;
   ontodebug:type "false"^^xsd:boolean
 ] .

[ ontodebug:axiom "hasFRU Domain Product"^^xsd:string ;
   ontodebug:type "false"^^xsd:boolean
 ] .

[ ontodebug:axiom "hasFRU Domain Product"^^xsd:string ;
   ontodebug:type "false"^^xsd:boolean
 ] .

[ ontodebug:axiom "SPDX SubClassOf ManagedSystemElement"^^xsd:string ;
   ontodebug:type "true"^^xsd:boolean
 ] .

[ ontodebug:axiom "Classifications SubClassOf Product"^^xsd:string ;
   ontodebug:type "false"^^xsd:boolean
 ] .

[ ontodebug:axiom "OperatingStatus DisjointWith SoftwareIdentity"^^xsd:string ;
   ontodebug:type "true"^^xsd:boolean
 ] .

[ ontodebug:axiom "hasName Domain ManagedElement"^^xsd:string ;
   ontodebug:type "true"^^xsd:boolean
 ] .

[ ontodebug:axiom "ManagedSystemElement DisjointWith Product"^^xsd:string ;
   ontodebug:type "true"^^xsd:boolean
 ] .

[ ontodebug:axiom "hasName Domain ManagedElement"^^xsd:string ;
   ontodebug:type "true"^^xsd:boolean
 ] .

[ ontodebug:axiom "FRU SubClassOf ManagedSystemElement"^^xsd:string ;
   ontodebug:type "false"^^xsd:boolean
 ] .

[ ontodebug:axiom "Unknown Type Classifications"^^xsd:string ;
   ontodebug:type "true"^^xsd:boolean
 ] .

[ ontodebug:axiom "Name Domain ManagedElement"^^xsd:string ;
   ontodebug:type "true"^^xsd:boolean
 ] .

[ ontodebug:axiom "hasProduct Range ManagedSystemElement"^^xsd:string ;
   ontodebug:type "true"^^xsd:boolean
 ] .

[ ontodebug:axiom "hasName Domain ManagedSystemElement"^^xsd:string ;
   ontodebug:type "true"^^xsd:boolean
 ] .

[ ontodebug:axiom "Caption Domain FRU"^^xsd:string ;
   ontodebug:type "true"^^xsd:boolean
 ] .

[ ontodebug:axiom "hasName Domain ManagedElement"^^xsd:string ;
   ontodebug:type "true"^^xsd:boolean
 ] .

[ ontodebug:axiom "Product SubClassOf ManagedSystemElement"^^xsd:string ;
   ontodebug:type "false"^^xsd:boolean
 ] .

[ ontodebug:axiom "Family Domain FRU"^^xsd:string ;
   ontodebug:type "false"^^xsd:boolean
 ] .

[ ontodebug:axiom "Classifications DisjointWith OperatingStatus"^^xsd:string ;
   ontodebug:type "true"^^xsd:boolean
 ] .

[ ontodebug:axiom "hasProduct Range SPDX"^^xsd:string ;
   ontodebug:type "true"^^xsd:boolean
 ] .

[ ontodebug:axiom "hasFRU Range FRU"^^xsd:string ;
   ontodebug:type "true"^^xsd:boolean
 ] .

[ ontodebug:axiom "WarrantyDuration Domain SPDX"^^xsd:string ;
   ontodebug:type "false"^^xsd:boolean
 ] .

[ ontodebug:axiom "OperatingStatus Domain PhysicalElement"^^xsd:string ;
   ontodebug:type "true"^^xsd:boolean
 ] .

[ ontodebug:axiom "hasName Domain ManagedSystemElement"^^xsd:string ;
   ontodebug:type "true"^^xsd:boolean
 ] .

[ ontodebug:axiom "SoftwareCreator Domain PhysicalElement"^^xsd:string ;
   ontodebug:type "false"^^xsd:boolean
 ] .

[ ontodebug:axiom "FRU SubClassOf ManagedSystemElement"^^xsd:string ;
   ontodebug:type "false"^^xsd:boolean
 ] .

[ ontodebug:axiom "FRU DisjointWith ManagedSystemElement"^^xsd:string ;
   ontodebug:type "true"^^xsd:boolean
 ] .

[ ontodebug:axiom "hasFRU Domain Product"^^xsd:string ;
   ontodebug:type "false"^^xsd:boolean
 ] .

[ ontodebug:axiom "hasName Domain ManagedElement"^^xsd:string ;
   ontodebug:type "true"^^xsd:boolean
 ] .

[ ontodebug:axiom "Caption Domain Location"^^xsd:string ;
   ontodebug:type "true"^^xsd:boolean
 ] .

[ ontodebug:axiom "Classifications SubClassOf Product"^^xsd:string ;
   ontodebug:type "false"^^xsd:boolean
 ] .

[ ontodebug:axiom "Location DisjointWith ManagedSystemElement"^^xsd:string ;
   ontodebug:type "true"^^xsd:boolean
 ] .

[ ontodebug:axiom "Caption Domain FRU"^^xsd:string ;
   ontodebug:type "true"^^xsd:boolean
 ] .

[ ontodebug:axiom "FRU DisjointWith SPDX"^^xsd:string ;
   ontodebug:type "true"^^xsd:boolean
 ] .

[ ontodebug:axiom "hasProduct Range SPDX"^^xsd:string ;
   ontodebug:type "true"^^xsd:boolean
 ] .

[ ontodebug:axiom "hasProduct Range SPDX"^^xsd:string ;
   ontodebug:type "true"^^xsd:boolean
 ] .

[ ontodebug:axiom "Product SubClassOf ManagedSystemElement"^^xsd:string ;
   ontodebug:type "false"^^xsd:boolean
 ] .

[ ontodebug:axiom "hasProduct Range SPDX"^^xsd:string ;
   ontodebug:type "true"^^xsd:boolean
 ] .

[ ontodebug:axiom "OperatingStatus Domain PhysicalElement"^^xsd:string ;
   ontodebug:type "true"^^xsd:boolean
 ] .

[ ontodebug:axiom "hasName Domain ManagedElement"^^xsd:string ;
   ontodebug:type "true"^^xsd:boolean
 ] .

[ ontodebug:axiom "Classifications DisjointWith OperatingStatus"^^xsd:string ;
   ontodebug:type "true"^^xsd:boolean
 ] .

[ ontodebug:axiom "hasProduct Range ManagedElement"^^xsd:string ;
   ontodebug:type "true"^^xsd:boolean
 ] .

[ ontodebug:axiom "Family Domain FRU"^^xsd:string ;
   ontodebug:type "false"^^xsd:boolean
 ] .

[ ontodebug:axiom "FRU and Product SubClassOf ManagedElement"^^xsd:string ;
   ontodebug:type "true"^^xsd:boolean
 ] .

[ ontodebug:axiom "hasProduct Range PhysicalElement"^^xsd:string ;
   ontodebug:type "true"^^xsd:boolean
 ] .

[ ontodebug:axiom "FRU DisjointWith ManagedSystemElement"^^xsd:string ;
   ontodebug:type "true"^^xsd:boolean
 ] .

[ ontodebug:axiom "WarrantyDuration Domain SPDX"^^xsd:string ;
   ontodebug:type "false"^^xsd:boolean
 ] .

[ ontodebug:axiom "hasFRU Range Product"^^xsd:string ;
   ontodebug:type "false"^^xsd:boolean
 ] .

[ ontodebug:axiom "WarrantyDuration Domain SoftwareIdentity"^^xsd:string ;
   ontodebug:type "false"^^xsd:boolean
 ] .

[ ontodebug:axiom "Product SubClassOf ManagedSystemElement"^^xsd:string ;
   ontodebug:type "false"^^xsd:boolean
 ] .

[ ontodebug:axiom "SPDX EquivalentTo SWID"^^xsd:string ;
   ontodebug:type "false"^^xsd:boolean
 ] .

[ ontodebug:axiom "ManagedSystemElement DisjointWith Product"^^xsd:string ;
   ontodebug:type "true"^^xsd:boolean
 ] .

[ ontodebug:axiom "hasProduct Range ManagedSystemElement"^^xsd:string ;
   ontodebug:type "true"^^xsd:boolean
 ] .

[ ontodebug:axiom "FRU SubClassOf ManagedSystemElement"^^xsd:string ;
   ontodebug:type "false"^^xsd:boolean
 ] .

[ ontodebug:axiom "hasName Domain ManagedSystemElement"^^xsd:string ;
   ontodebug:type "true"^^xsd:boolean
 ] .

[ ontodebug:axiom "Classifications DisjointWith OperatingStatus"^^xsd:string ;
   ontodebug:type "true"^^xsd:boolean
 ] .

[ ontodebug:axiom "Manufacturer Domain SoftwareIdentity"^^xsd:string ;
   ontodebug:type "false"^^xsd:boolean
 ] .

[ ontodebug:axiom "hasFRU Domain Product"^^xsd:string ;
   ontodebug:type "false"^^xsd:boolean
 ] .

[ ontodebug:axiom "Product SubClassOf ManagedSystemElement"^^xsd:string ;
   ontodebug:type "false"^^xsd:boolean
 ] .

[ ontodebug:axiom "Product DisjointWith SoftwareIdentity"^^xsd:string ;
   ontodebug:type "true"^^xsd:boolean
 ] .

[ ontodebug:axiom "hasName Domain ManagedSystemElement"^^xsd:string ;
   ontodebug:type "true"^^xsd:boolean
 ] .

[ ontodebug:axiom "Manufacturer Domain ManagedElement"^^xsd:string ;
   ontodebug:type "true"^^xsd:boolean
 ] .

[ ontodebug:axiom "Name Domain PhysicalElement"^^xsd:string ;
   ontodebug:type "true"^^xsd:boolean
 ] .

[ ontodebug:axiom "Classifications SubClassOf Product"^^xsd:string ;
   ontodebug:type "false"^^xsd:boolean
 ] .

[ ontodebug:axiom "CISCO_CATALYST_3750 Caption \"Cisco Catalyst 3750\"^^string"^^xsd:string ;
   ontodebug:type "true"^^xsd:boolean
 ] .

[ ontodebug:axiom "SPDX SubClassOf ManagedSystemElement"^^xsd:string ;
   ontodebug:type "true"^^xsd:boolean
 ] .

[ ontodebug:axiom "Location DisjointWith ManagedSystemElement"^^xsd:string ;
   ontodebug:type "true"^^xsd:boolean
 ] .

[ ontodebug:axiom "hasName Domain ManagedElement"^^xsd:string ;
   ontodebug:type "true"^^xsd:boolean
 ] .

[ ontodebug:axiom "hasName Domain ManagedElement"^^xsd:string ;
   ontodebug:type "true"^^xsd:boolean
 ] .

[ ontodebug:axiom "OperatingStatus Domain PhysicalElement"^^xsd:string ;
   ontodebug:type "true"^^xsd:boolean
 ] .

[ ontodebug:axiom "hasName Domain ManagedSystemElement"^^xsd:string ;
   ontodebug:type "true"^^xsd:boolean
 ] .

[ ontodebug:axiom "hasProduct Range ManagedSystemElement"^^xsd:string ;
   ontodebug:type "true"^^xsd:boolean
 ] .

[ ontodebug:axiom "Unknown Type Classifications"^^xsd:string ;
   ontodebug:type "true"^^xsd:boolean
 ] .

[ ontodebug:axiom "hasProduct Range FRU"^^xsd:string ;
   ontodebug:type "true"^^xsd:boolean
 ] .

[ ontodebug:axiom "SPDX SubClassOf ManagedSystemElement"^^xsd:string ;
   ontodebug:type "true"^^xsd:boolean
 ] .

[ ontodebug:axiom "hasLocation Range SoftwareIdentity"^^xsd:string ;
   ontodebug:type "false"^^xsd:boolean
 ] .

[ ontodebug:axiom "OperatingStatus Domain PhysicalElement"^^xsd:string ;
   ontodebug:type "true"^^xsd:boolean
 ] .

[ ontodebug:axiom "FRU and Product SubClassOf ManagedElement"^^xsd:string ;
   ontodebug:type "true"^^xsd:boolean
 ] .

[ ontodebug:axiom "hasProduct Range ManagedElement"^^xsd:string ;
   ontodebug:type "true"^^xsd:boolean
 ] .

[ ontodebug:axiom "hasProduct Range ManagedSystemElement"^^xsd:string ;
   ontodebug:type "true"^^xsd:boolean
 ] .

[ ontodebug:axiom "hasFRU Domain Product"^^xsd:string ;
   ontodebug:type "false"^^xsd:boolean
 ] .

[ ontodebug:axiom "WarrantyDuration Domain SoftwareIdentity"^^xsd:string ;
   ontodebug:type "false"^^xsd:boolean
 ] .

[ ontodebug:axiom "hasProduct Range ManagedElement"^^xsd:string ;
   ontodebug:type "true"^^xsd:boolean
 ] .

[ ontodebug:axiom "hasProduct Range ManagedSystemElement"^^xsd:string ;
   ontodebug:type "true"^^xsd:boolean
 ] .

[ ontodebug:axiom "hasProduct Range FRU"^^xsd:string ;
   ontodebug:type "true"^^xsd:boolean
 ] .

[ ontodebug:axiom "hasProduct Range ManagedElement"^^xsd:string ;
   ontodebug:type "true"^^xsd:boolean
 ] .

[ ontodebug:axiom "Location SubClassOf ManagedSystemElement"^^xsd:string ;
   ontodebug:type "false"^^xsd:boolean
 ] .

[ ontodebug:axiom "FRU DisjointWith ManagedSystemElement"^^xsd:string ;
   ontodebug:type "true"^^xsd:boolean
 ] .

[ ontodebug:axiom "hasFRU Range FRU"^^xsd:string ;
   ontodebug:type "true"^^xsd:boolean
 ] .

[ ontodebug:axiom "SPDX SubClassOf ManagedSystemElement"^^xsd:string ;
   ontodebug:type "true"^^xsd:boolean
 ] .

[ ontodebug:axiom "Caption Domain FRU"^^xsd:string ;
   ontodebug:type "true"^^xsd:boolean
 ] .

[ ontodebug:axiom "SPDX EquivalentTo SWID"^^xsd:string ;
   ontodebug:type "false"^^xsd:boolean
 ] .

[ ontodebug:axiom "SPDX SubClassOf ManagedSystemElement"^^xsd:string ;
   ontodebug:type "true"^^xsd:boolean
 ] .

[ ontodebug:axiom "Unknown Type Classifications"^^xsd:string ;
   ontodebug:type "true"^^xsd:boolean
 ] .

[ ontodebug:axiom "hasProduct Range SPDX"^^xsd:string ;
   ontodebug:type "true"^^xsd:boolean
 ] .

[ ontodebug:axiom "Product DisjointWith SoftwareIdentity"^^xsd:string ;
   ontodebug:type "true"^^xsd:boolean
 ] .

[ ontodebug:axiom "Product SubClassOf ManagedSystemElement"^^xsd:string ;
   ontodebug:type "false"^^xsd:boolean
 ] .

[ ontodebug:axiom "Product DisjointWith SoftwareIdentity"^^xsd:string ;
   ontodebug:type "true"^^xsd:boolean
 ] .

[ ontodebug:axiom "hasName Domain ManagedElement"^^xsd:string ;
   ontodebug:type "true"^^xsd:boolean
 ] .

[ ontodebug:axiom "hasName Domain ManagedElement"^^xsd:string ;
   ontodebug:type "true"^^xsd:boolean
 ] .

[ ontodebug:axiom "ManagedSystemElement DisjointWith Product"^^xsd:string ;
   ontodebug:type "true"^^xsd:boolean
 ] .

[ ontodebug:axiom "hasLocation Range SoftwareIdentity"^^xsd:string ;
   ontodebug:type "false"^^xsd:boolean
 ] .

[ ontodebug:axiom "Caption Domain Location"^^xsd:string ;
   ontodebug:type "true"^^xsd:boolean
 ] .

[ ontodebug:axiom "hasFRU Range Product"^^xsd:string ;
   ontodebug:type "false"^^xsd:boolean
 ] .

[ ontodebug:axiom "FRU and Product SubClassOf ManagedElement"^^xsd:string ;
   ontodebug:type "true"^^xsd:boolean
 ] .

[ ontodebug:axiom "WarrantyDuration Domain SPDX"^^xsd:string ;
   ontodebug:type "false"^^xsd:boolean
 ] .

[ ontodebug:axiom "SerialNumber Domain PhysicalElement"^^xsd:string ;
   ontodebug:type "true"^^xsd:boolean
 ] .

[ ontodebug:axiom "hasFRU Range FRU"^^xsd:string ;
   ontodebug:type "true"^^xsd:boolean
 ] .

[ ontodebug:axiom "Caption Domain Location"^^xsd:string ;
   ontodebug:type "true"^^xsd:boolean
 ] .

[ ontodebug:axiom "FRU and Product SubClassOf ManagedElement"^^xsd:string ;
   ontodebug:type "true"^^xsd:boolean
 ] .

[ ontodebug:axiom "WarrantyDuration Domain SoftwareIdentity"^^xsd:string ;
   ontodebug:type "false"^^xsd:boolean
 ] .

[ ontodebug:axiom "FRU SubClassOf ManagedSystemElement"^^xsd:string ;
   ontodebug:type "false"^^xsd:boolean
 ] .

[ ontodebug:axiom "hasName Domain ManagedSystemElement"^^xsd:string ;
   ontodebug:type "true"^^xsd:boolean
 ] .

[ ontodebug:axiom "hasFRU Range Product"^^xsd:string ;
   ontodebug:type "false"^^xsd:boolean
 ] .

[ ontodebug:axiom "FRU DisjointWith ManagedSystemElement"^^xsd:string ;
   ontodebug:type "true"^^xsd:boolean
 ] .

[ ontodebug:axiom "WarrantyDuration Domain SoftwareIdentity"^^xsd:string ;
   ontodebug:type "false"^^xsd:boolean
 ] .

[ ontodebug:axiom "hasProduct Range PhysicalElement"^^xsd:string ;
   ontodebug:type "true"^^xsd:boolean
 ] .

[ ontodebug:axiom "OperatingStatus DisjointWith SoftwareIdentity"^^xsd:string ;
   ontodebug:type "true"^^xsd:boolean
 ] .

[ ontodebug:axiom "Family Domain FRU"^^xsd:string ;
   ontodebug:type "false"^^xsd:boolean
 ] .

[ ontodebug:axiom "Caption Domain Location"^^xsd:string ;
   ontodebug:type "true"^^xsd:boolean
 ] .

[ ontodebug:axiom "Manufacturer Domain SoftwareIdentity"^^xsd:string ;
   ontodebug:type "false"^^xsd:boolean
 ] .

[ ontodebug:axiom "hasName Domain ManagedElement"^^xsd:string ;
   ontodebug:type "true"^^xsd:boolean
 ] .

[ ontodebug:axiom "Location SubClassOf ManagedSystemElement"^^xsd:string ;
   ontodebug:type "false"^^xsd:boolean
 ] .

[ ontodebug:axiom "hasProduct Range SoftwareIdentity"^^xsd:string ;
   ontodebug:type "true"^^xsd:boolean
 ] .

[ ontodebug:axiom "hasName Domain ManagedElement"^^xsd:string ;
   ontodebug:type "true"^^xsd:boolean
 ] .

[ ontodebug:axiom "WarrantyDuration Domain SoftwareIdentity"^^xsd:string ;
   ontodebug:type "false"^^xsd:boolean
 ] .

[ ontodebug:axiom "SPDX EquivalentTo SWID"^^xsd:string ;
   ontodebug:type "false"^^xsd:boolean
 ] .

[ ontodebug:axiom "Product DisjointWith SoftwareIdentity"^^xsd:string ;
   ontodebug:type "true"^^xsd:boolean
 ] .

[ ontodebug:axiom "hasName Domain ManagedElement"^^xsd:string ;
   ontodebug:type "true"^^xsd:boolean
 ] .

[ ontodebug:axiom "Name Domain ManagedElement"^^xsd:string ;
   ontodebug:type "true"^^xsd:boolean
 ] .

[ ontodebug:axiom "FRU DisjointWith ManagedSystemElement"^^xsd:string ;
   ontodebug:type "true"^^xsd:boolean
 ] .

[ ontodebug:axiom "Location SubClassOf ManagedSystemElement"^^xsd:string ;
   ontodebug:type "false"^^xsd:boolean
 ] .

[ ontodebug:axiom "SPDX EquivalentTo SWID"^^xsd:string ;
   ontodebug:type "false"^^xsd:boolean
 ] .

[ ontodebug:axiom "hasName Domain ManagedElement"^^xsd:string ;
   ontodebug:type "true"^^xsd:boolean
 ] .

[ ontodebug:axiom "hasName Domain ManagedSystemElement"^^xsd:string ;
   ontodebug:type "true"^^xsd:boolean
 ] .

[ ontodebug:axiom "hasProduct Range FRU"^^xsd:string ;
   ontodebug:type "true"^^xsd:boolean
 ] .

[ ontodebug:axiom "hasLocation Range SoftwareIdentity"^^xsd:string ;
   ontodebug:type "false"^^xsd:boolean
 ] .

[ ontodebug:axiom "hasFRU Range Product"^^xsd:string ;
   ontodebug:type "false"^^xsd:boolean
 ] .

[ ontodebug:axiom "hasName Domain ManagedSystemElement"^^xsd:string ;
   ontodebug:type "true"^^xsd:boolean
 ] .

[ ontodebug:axiom "Location SubClassOf ManagedSystemElement"^^xsd:string ;
   ontodebug:type "false"^^xsd:boolean
 ] .

[ ontodebug:axiom "FRU SubClassOf ManagedSystemElement"^^xsd:string ;
   ontodebug:type "false"^^xsd:boolean
 ] .

[ ontodebug:axiom "Product SubClassOf ManagedSystemElement"^^xsd:string ;
   ontodebug:type "false"^^xsd:boolean
 ] .

[ ontodebug:axiom "OperatingStatus Domain PhysicalElement"^^xsd:string ;
   ontodebug:type "true"^^xsd:boolean
 ] .

[ ontodebug:axiom "hasFRU Range FRU"^^xsd:string ;
   ontodebug:type "true"^^xsd:boolean
 ] .

[ ontodebug:axiom "FRU DisjointWith ManagedSystemElement"^^xsd:string ;
   ontodebug:type "true"^^xsd:boolean
 ] .

[ ontodebug:axiom "hasName Domain ManagedSystemElement"^^xsd:string ;
   ontodebug:type "true"^^xsd:boolean
 ] .

[ ontodebug:axiom "hasProduct Range PhysicalElement"^^xsd:string ;
   ontodebug:type "true"^^xsd:boolean
 ] .

[ ontodebug:axiom "OperatingStatus DisjointWith SoftwareIdentity"^^xsd:string ;
   ontodebug:type "true"^^xsd:boolean
 ] .

[ ontodebug:axiom "hasProduct Range SoftwareIdentity"^^xsd:string ;
   ontodebug:type "true"^^xsd:boolean
 ] .

[ ontodebug:axiom "Manufacturer Domain SoftwareIdentity"^^xsd:string ;
   ontodebug:type "false"^^xsd:boolean
 ] .

[ ontodebug:axiom "ManagedSystemElement DisjointWith Product"^^xsd:string ;
   ontodebug:type "true"^^xsd:boolean
 ] .

[ ontodebug:axiom "Manufacturer Domain ManagedElement"^^xsd:string ;
   ontodebug:type "true"^^xsd:boolean
 ] .

[ ontodebug:axiom "hasProduct Range FRU"^^xsd:string ;
   ontodebug:type "true"^^xsd:boolean
 ] .

[ ontodebug:axiom "Family Domain FRU"^^xsd:string ;
   ontodebug:type "false"^^xsd:boolean
 ] .

[ ontodebug:axiom "Location DisjointWith ManagedSystemElement"^^xsd:string ;
   ontodebug:type "true"^^xsd:boolean
 ] .

[ ontodebug:axiom "SoftwareCreator Domain PhysicalElement"^^xsd:string ;
   ontodebug:type "false"^^xsd:boolean
 ] .

[ ontodebug:axiom "hasName Domain ManagedElement"^^xsd:string ;
   ontodebug:type "true"^^xsd:boolean
 ] .

[ ontodebug:axiom "hasFRU Range FRU"^^xsd:string ;
   ontodebug:type "true"^^xsd:boolean
 ] .

[ ontodebug:axiom "Manufacturer Domain SoftwareIdentity"^^xsd:string ;
   ontodebug:type "false"^^xsd:boolean
 ] .

[ ontodebug:axiom "hasName Domain ManagedSystemElement"^^xsd:string ;
   ontodebug:type "true"^^xsd:boolean
 ] .

[ ontodebug:axiom "Location DisjointWith ManagedSystemElement"^^xsd:string ;
   ontodebug:type "true"^^xsd:boolean
 ] .

[ ontodebug:axiom "Product SubClassOf ManagedSystemElement"^^xsd:string ;
   ontodebug:type "false"^^xsd:boolean
 ] .

[ ontodebug:axiom "FRU SubClassOf ManagedSystemElement"^^xsd:string ;
   ontodebug:type "false"^^xsd:boolean
 ] .

[ ontodebug:axiom "SPDX SubClassOf ManagedSystemElement"^^xsd:string ;
   ontodebug:type "true"^^xsd:boolean
 ] .

[ ontodebug:axiom "FRU and Product SubClassOf ManagedElement"^^xsd:string ;
   ontodebug:type "true"^^xsd:boolean
 ] .

[ ontodebug:axiom "hasProduct Range ManagedElement"^^xsd:string ;
   ontodebug:type "true"^^xsd:boolean
 ] .

[ ontodebug:axiom "Location SubClassOf ManagedSystemElement"^^xsd:string ;
   ontodebug:type "false"^^xsd:boolean
 ] .

[ ontodebug:axiom "SPDX EquivalentTo SWID"^^xsd:string ;
   ontodebug:type "false"^^xsd:boolean
 ] .

[ ontodebug:axiom "hasProduct Range FRU"^^xsd:string ;
   ontodebug:type "true"^^xsd:boolean
 ] .

[ ontodebug:axiom "hasProduct Range FRU"^^xsd:string ;
   ontodebug:type "true"^^xsd:boolean
 ] .

[ ontodebug:axiom "Unknown Type Classifications"^^xsd:string ;
   ontodebug:type "true"^^xsd:boolean
 ] .

[ ontodebug:axiom "Product SubClassOf ManagedSystemElement"^^xsd:string ;
   ontodebug:type "false"^^xsd:boolean
 ] .

[ ontodebug:axiom "CISCO_CATALYST_3750 Caption \"Cisco Catalyst 3750\"^^string"^^xsd:string ;
   ontodebug:type "true"^^xsd:boolean
 ] .

[ ontodebug:axiom "Manufacturer Domain SoftwareIdentity"^^xsd:string ;
   ontodebug:type "false"^^xsd:boolean
 ] .

[ ontodebug:axiom "hasFRU Range FRU"^^xsd:string ;
   ontodebug:type "true"^^xsd:boolean
 ] .

[ ontodebug:axiom "Caption Domain Location"^^xsd:string ;
   ontodebug:type "true"^^xsd:boolean
 ] .

[ ontodebug:axiom "Product SubClassOf ManagedSystemElement"^^xsd:string ;
   ontodebug:type "false"^^xsd:boolean
 ] .

[ ontodebug:axiom "WarrantyDuration Domain SPDX"^^xsd:string ;
   ontodebug:type "false"^^xsd:boolean
 ] .

[ ontodebug:axiom "OperatingStatus Domain PhysicalElement"^^xsd:string ;
   ontodebug:type "true"^^xsd:boolean
 ] .

[ ontodebug:axiom "hasProduct Range ManagedElement"^^xsd:string ;
   ontodebug:type "true"^^xsd:boolean
 ] .

[ ontodebug:axiom "hasLocation Range SoftwareIdentity"^^xsd:string ;
   ontodebug:type "false"^^xsd:boolean
 ] .

[ ontodebug:axiom "Classifications SubClassOf Product"^^xsd:string ;
   ontodebug:type "false"^^xsd:boolean
 ] .

[ ontodebug:axiom "hasLocation Range SoftwareIdentity"^^xsd:string ;
   ontodebug:type "false"^^xsd:boolean
 ] .

[ ontodebug:axiom "FRU DisjointWith SPDX"^^xsd:string ;
   ontodebug:type "true"^^xsd:boolean
 ] .

[ ontodebug:axiom "hasName Domain ManagedElement"^^xsd:string ;
   ontodebug:type "true"^^xsd:boolean
 ] .

[ ontodebug:axiom "Product DisjointWith SoftwareIdentity"^^xsd:string ;
   ontodebug:type "true"^^xsd:boolean
 ] .

[ ontodebug:axiom "FRU SubClassOf ManagedSystemElement"^^xsd:string ;
   ontodebug:type "false"^^xsd:boolean
 ] .

[ ontodebug:axiom "FRU DisjointWith ManagedSystemElement"^^xsd:string ;
   ontodebug:type "true"^^xsd:boolean
 ] .

[ ontodebug:axiom "Name Domain PhysicalElement"^^xsd:string ;
   ontodebug:type "true"^^xsd:boolean
 ] .

[ ontodebug:axiom "hasFRU Range Product"^^xsd:string ;
   ontodebug:type "false"^^xsd:boolean
 ] .

[ ontodebug:axiom "Unknown Type Classifications"^^xsd:string ;
   ontodebug:type "true"^^xsd:boolean
 ] .

[ ontodebug:axiom "Product DisjointWith SoftwareIdentity"^^xsd:string ;
   ontodebug:type "true"^^xsd:boolean
 ] .

[ ontodebug:axiom "hasProduct Range SoftwareIdentity"^^xsd:string ;
   ontodebug:type "true"^^xsd:boolean
 ] .

[ ontodebug:axiom "hasName Domain ManagedSystemElement"^^xsd:string ;
   ontodebug:type "true"^^xsd:boolean
 ] .

[ ontodebug:axiom "hasName Domain ManagedElement"^^xsd:string ;
   ontodebug:type "true"^^xsd:boolean
 ] .

[ ontodebug:axiom "FRU DisjointWith SPDX"^^xsd:string ;
   ontodebug:type "true"^^xsd:boolean
 ] .

[ ontodebug:axiom "hasLocation Range SoftwareIdentity"^^xsd:string ;
   ontodebug:type "false"^^xsd:boolean
 ] .

[ ontodebug:axiom "FRU SubClassOf ManagedSystemElement"^^xsd:string ;
   ontodebug:type "false"^^xsd:boolean
 ] .

[ ontodebug:axiom "Location DisjointWith ManagedSystemElement"^^xsd:string ;
   ontodebug:type "true"^^xsd:boolean
 ] .

[ ontodebug:axiom "hasName Domain ManagedSystemElement"^^xsd:string ;
   ontodebug:type "true"^^xsd:boolean
 ] .

[ ontodebug:axiom "hasLocation Range SoftwareIdentity"^^xsd:string ;
   ontodebug:type "false"^^xsd:boolean
 ] .

[ ontodebug:axiom "hasName Domain ManagedSystemElement"^^xsd:string ;
   ontodebug:type "true"^^xsd:boolean
 ] .

[ ontodebug:axiom "Product DisjointWith SoftwareIdentity"^^xsd:string ;
   ontodebug:type "true"^^xsd:boolean
 ] .

[ ontodebug:axiom "Manufacturer Domain SoftwareIdentity"^^xsd:string ;
   ontodebug:type "false"^^xsd:boolean
 ] .

[ ontodebug:axiom "Classifications DisjointWith OperatingStatus"^^xsd:string ;
   ontodebug:type "true"^^xsd:boolean
 ] .

[ ontodebug:axiom "Unknown Type Classifications"^^xsd:string ;
   ontodebug:type "true"^^xsd:boolean
 ] .

[ ontodebug:axiom "WarrantyDuration Domain SPDX"^^xsd:string ;
   ontodebug:type "false"^^xsd:boolean
 ] .

[ ontodebug:axiom "WarrantyDuration Domain SoftwareIdentity"^^xsd:string ;
   ontodebug:type "false"^^xsd:boolean
 ] .

[ ontodebug:axiom "SerialNumber Domain PhysicalElement"^^xsd:string ;
   ontodebug:type "true"^^xsd:boolean
 ] .

[ ontodebug:axiom "FRU SubClassOf ManagedSystemElement"^^xsd:string ;
   ontodebug:type "false"^^xsd:boolean
 ] .

[ ontodebug:axiom "Classifications SubClassOf Product"^^xsd:string ;
   ontodebug:type "false"^^xsd:boolean
 ] .

[ ontodebug:axiom "hasFRU Range FRU"^^xsd:string ;
   ontodebug:type "true"^^xsd:boolean
 ] .

[ ontodebug:axiom "OperatingStatus DisjointWith SoftwareIdentity"^^xsd:string ;
   ontodebug:type "true"^^xsd:boolean
 ] .

[ ontodebug:axiom "Manufacturer Domain ManagedElement"^^xsd:string ;
   ontodebug:type "true"^^xsd:boolean
 ] .

[ ontodebug:axiom "FRU DisjointWith SPDX"^^xsd:string ;
   ontodebug:type "true"^^xsd:boolean
 ] .

[ ontodebug:axiom "SPDX SubClassOf ManagedSystemElement"^^xsd:string ;
   ontodebug:type "true"^^xsd:boolean
 ] .

[ ontodebug:axiom "hasName Domain ManagedElement"^^xsd:string ;
   ontodebug:type "true"^^xsd:boolean
 ] .

[ ontodebug:axiom "Product SubClassOf ManagedSystemElement"^^xsd:string ;
   ontodebug:type "false"^^xsd:boolean
 ] .

[ ontodebug:axiom "Product SubClassOf ManagedSystemElement"^^xsd:string ;
   ontodebug:type "false"^^xsd:boolean
 ] .

[ ontodebug:axiom "FRU SubClassOf ManagedSystemElement"^^xsd:string ;
   ontodebug:type "false"^^xsd:boolean
 ] .

[ ontodebug:axiom "FRU DisjointWith SPDX"^^xsd:string ;
   ontodebug:type "true"^^xsd:boolean
 ] .

[ ontodebug:axiom "FRU DisjointWith ManagedSystemElement"^^xsd:string ;
   ontodebug:type "true"^^xsd:boolean
 ] .

[ ontodebug:axiom "hasFRU Range Product"^^xsd:string ;
   ontodebug:type "false"^^xsd:boolean
 ] .

[ ontodebug:axiom "FRU and Product SubClassOf ManagedElement"^^xsd:string ;
   ontodebug:type "true"^^xsd:boolean
 ] .

[ ontodebug:axiom "SPDX EquivalentTo SWID"^^xsd:string ;
   ontodebug:type "false"^^xsd:boolean
 ] .

[ ontodebug:axiom "FRU SubClassOf ManagedSystemElement"^^xsd:string ;
   ontodebug:type "false"^^xsd:boolean
 ] .

[ ontodebug:axiom "hasName Domain ManagedElement"^^xsd:string ;
   ontodebug:type "true"^^xsd:boolean
 ] .

[ ontodebug:axiom "SPDX SubClassOf ManagedSystemElement"^^xsd:string ;
   ontodebug:type "true"^^xsd:boolean
 ] .

[ ontodebug:axiom "Caption Domain FRU"^^xsd:string ;
   ontodebug:type "true"^^xsd:boolean
 ] .

[ ontodebug:axiom "FRU DisjointWith ManagedSystemElement"^^xsd:string ;
   ontodebug:type "true"^^xsd:boolean
 ] .

[ ontodebug:axiom "OperatingStatus Domain PhysicalElement"^^xsd:string ;
   ontodebug:type "true"^^xsd:boolean
 ] .

[ ontodebug:axiom "hasProduct Range PhysicalElement"^^xsd:string ;
   ontodebug:type "true"^^xsd:boolean
 ] .

[ ontodebug:axiom "ManagedSystemElement DisjointWith Product"^^xsd:string ;
   ontodebug:type "true"^^xsd:boolean
 ] .

[ ontodebug:axiom "Product SubClassOf ManagedSystemElement"^^xsd:string ;
   ontodebug:type "false"^^xsd:boolean
 ] .

[ ontodebug:axiom "Classifications SubClassOf Product"^^xsd:string ;
   ontodebug:type "false"^^xsd:boolean
 ] .

[ ontodebug:axiom "hasFRU Range FRU"^^xsd:string ;
   ontodebug:type "true"^^xsd:boolean
 ] .

[ ontodebug:axiom "Manufacturer Domain SoftwareIdentity"^^xsd:string ;
   ontodebug:type "false"^^xsd:boolean
 ] .

[ ontodebug:axiom "hasFRU Range FRU"^^xsd:string ;
   ontodebug:type "true"^^xsd:boolean
 ] .

[ ontodebug:axiom "hasFRU Domain Product"^^xsd:string ;
   ontodebug:type "false"^^xsd:boolean
 ] .

[ ontodebug:axiom "hasFRU Range Product"^^xsd:string ;
   ontodebug:type "false"^^xsd:boolean
 ] .

[ ontodebug:axiom "Family Domain FRU"^^xsd:string ;
   ontodebug:type "false"^^xsd:boolean
 ] .

[ ontodebug:axiom "hasFRU Domain Product"^^xsd:string ;
   ontodebug:type "false"^^xsd:boolean
 ] .

[ ontodebug:axiom "Unknown Type Classifications"^^xsd:string ;
   ontodebug:type "true"^^xsd:boolean
 ] .

[ ontodebug:axiom "Location DisjointWith ManagedSystemElement"^^xsd:string ;
   ontodebug:type "true"^^xsd:boolean
 ] .

[ ontodebug:axiom "Classifications DisjointWith OperatingStatus"^^xsd:string ;
   ontodebug:type "true"^^xsd:boolean
 ] .

[ ontodebug:axiom "ManagedSystemElement DisjointWith Product"^^xsd:string ;
   ontodebug:type "true"^^xsd:boolean
 ] .

[ ontodebug:axiom "Product SubClassOf ManagedSystemElement"^^xsd:string ;
   ontodebug:type "false"^^xsd:boolean
 ] .

[ ontodebug:axiom "hasFRU Domain Product"^^xsd:string ;
   ontodebug:type "false"^^xsd:boolean
 ] .

[ ontodebug:axiom "hasFRU Domain Product"^^xsd:string ;
   ontodebug:type "false"^^xsd:boolean
 ] .

[ ontodebug:axiom "hasName Domain ManagedSystemElement"^^xsd:string ;
   ontodebug:type "true"^^xsd:boolean
 ] .

[ ontodebug:axiom "FRU DisjointWith ManagedSystemElement"^^xsd:string ;
   ontodebug:type "true"^^xsd:boolean
 ] .

[ ontodebug:axiom "WarrantyDuration Domain SPDX"^^xsd:string ;
   ontodebug:type "false"^^xsd:boolean
 ] .

[ ontodebug:axiom "ManagedSystemElement DisjointWith Product"^^xsd:string ;
   ontodebug:type "true"^^xsd:boolean
 ] .

[ ontodebug:axiom "hasLocation Range SoftwareIdentity"^^xsd:string ;
   ontodebug:type "false"^^xsd:boolean
 ] .

[ ontodebug:axiom "WarrantyDuration Domain SoftwareIdentity"^^xsd:string ;
   ontodebug:type "false"^^xsd:boolean
 ] .

[ ontodebug:axiom "OperatingStatus Domain PhysicalElement"^^xsd:string ;
   ontodebug:type "true"^^xsd:boolean
 ] .

[ ontodebug:axiom "FRU and Product SubClassOf ManagedElement"^^xsd:string ;
   ontodebug:type "true"^^xsd:boolean
 ] .

[ ontodebug:axiom "SPDX EquivalentTo SWID"^^xsd:string ;
   ontodebug:type "false"^^xsd:boolean
 ] .

[ ontodebug:axiom "hasProduct Range ManagedElement"^^xsd:string ;
   ontodebug:type "true"^^xsd:boolean
 ] .

[ ontodebug:axiom "WarrantyDuration Domain SPDX"^^xsd:string ;
   ontodebug:type "false"^^xsd:boolean
 ] .

[ ontodebug:axiom "hasProduct Range ManagedElement"^^xsd:string ;
   ontodebug:type "true"^^xsd:boolean
 ] .

[ ontodebug:axiom "hasProduct Range ManagedSystemElement"^^xsd:string ;
   ontodebug:type "true"^^xsd:boolean
 ] .

[ ontodebug:axiom "OperatingStatus DisjointWith SoftwareIdentity"^^xsd:string ;
   ontodebug:type "true"^^xsd:boolean
 ] .

[ ontodebug:axiom "Product DisjointWith SoftwareIdentity"^^xsd:string ;
   ontodebug:type "true"^^xsd:boolean
 ] .

[ ontodebug:axiom "WarrantyDuration Domain SPDX"^^xsd:string ;
   ontodebug:type "false"^^xsd:boolean
 ] .

[ ontodebug:axiom "hasName Domain ManagedSystemElement"^^xsd:string ;
   ontodebug:type "true"^^xsd:boolean
 ] .

[ ontodebug:axiom "hasFRU Range Product"^^xsd:string ;
   ontodebug:type "false"^^xsd:boolean
 ] .

[ ontodebug:axiom "hasProduct Range SoftwareIdentity"^^xsd:string ;
   ontodebug:type "true"^^xsd:boolean
 ] .

[ ontodebug:axiom "OperatingStatus DisjointWith SoftwareIdentity"^^xsd:string ;
   ontodebug:type "true"^^xsd:boolean
 ] .

[ ontodebug:axiom "OperatingStatus DisjointWith SoftwareIdentity"^^xsd:string ;
   ontodebug:type "true"^^xsd:boolean
 ] .

[ ontodebug:axiom "Family Domain FRU"^^xsd:string ;
   ontodebug:type "false"^^xsd:boolean
 ] .

[ ontodebug:axiom "hasFRU Range Product"^^xsd:string ;
   ontodebug:type "false"^^xsd:boolean
 ] .

[ ontodebug:axiom "hasName Domain ManagedElement"^^xsd:string ;
   ontodebug:type "true"^^xsd:boolean
 ] .

[ ontodebug:axiom "hasProduct Range PhysicalElement"^^xsd:string ;
   ontodebug:type "true"^^xsd:boolean
 ] .

[ ontodebug:axiom "SPDX SubClassOf ManagedSystemElement"^^xsd:string ;
   ontodebug:type "true"^^xsd:boolean
 ] .

[ ontodebug:axiom "Name Domain ManagedElement"^^xsd:string ;
   ontodebug:type "true"^^xsd:boolean
 ] .

[ ontodebug:axiom "SerialNumber Domain PhysicalElement"^^xsd:string ;
   ontodebug:type "true"^^xsd:boolean
 ] .

[ ontodebug:axiom "FRU SubClassOf ManagedSystemElement"^^xsd:string ;
   ontodebug:type "false"^^xsd:boolean
 ] .

[ ontodebug:axiom "Manufacturer Domain ManagedElement"^^xsd:string ;
   ontodebug:type "true"^^xsd:boolean
 ] .

[ ontodebug:axiom "CISCO_CATALYST_3750 Caption \"Cisco Catalyst 3750\"^^string"^^xsd:string ;
   ontodebug:type "true"^^xsd:boolean
 ] .

[ ontodebug:axiom "Name Domain PhysicalElement"^^xsd:string ;
   ontodebug:type "true"^^xsd:boolean
 ] .

[ ontodebug:axiom "SoftwareCreator Domain PhysicalElement"^^xsd:string ;
   ontodebug:type "false"^^xsd:boolean
 ] .

[ ontodebug:axiom "Manufacturer Domain SoftwareIdentity"^^xsd:string ;
   ontodebug:type "false"^^xsd:boolean
 ] .

[ ontodebug:axiom "hasName Domain ManagedElement"^^xsd:string ;
   ontodebug:type "true"^^xsd:boolean
 ] .

[ ontodebug:axiom "FRU SubClassOf ManagedSystemElement"^^xsd:string ;
   ontodebug:type "false"^^xsd:boolean
 ] .

[ ontodebug:axiom "Manufacturer Domain ManagedElement"^^xsd:string ;
   ontodebug:type "true"^^xsd:boolean
 ] .

[ ontodebug:axiom "FRU and Product SubClassOf ManagedElement"^^xsd:string ;
   ontodebug:type "true"^^xsd:boolean
 ] .

[ ontodebug:axiom "hasProduct Range ManagedElement"^^xsd:string ;
   ontodebug:type "true"^^xsd:boolean
 ] .

[ ontodebug:axiom "hasFRU Range Product"^^xsd:string ;
   ontodebug:type "false"^^xsd:boolean
 ] .

[ ontodebug:axiom "OperatingStatus Domain PhysicalElement"^^xsd:string ;
   ontodebug:type "true"^^xsd:boolean
 ] .

[ ontodebug:axiom "Classifications SubClassOf Product"^^xsd:string ;
   ontodebug:type "false"^^xsd:boolean
 ] .

[ ontodebug:axiom "WarrantyDuration Domain SPDX"^^xsd:string ;
   ontodebug:type "false"^^xsd:boolean
 ] .

[ ontodebug:axiom "WarrantyDuration Domain SoftwareIdentity"^^xsd:string ;
   ontodebug:type "false"^^xsd:boolean
 ] .

[ ontodebug:axiom "hasFRU Range FRU"^^xsd:string ;
   ontodebug:type "true"^^xsd:boolean
 ] .

[ ontodebug:axiom "hasFRU Range FRU"^^xsd:string ;
   ontodebug:type "true"^^xsd:boolean
 ] .

[ ontodebug:axiom "ManagedSystemElement DisjointWith Product"^^xsd:string ;
   ontodebug:type "true"^^xsd:boolean
 ] .

[ ontodebug:axiom "FRU SubClassOf ManagedSystemElement"^^xsd:string ;
   ontodebug:type "false"^^xsd:boolean
 ] .

[ ontodebug:axiom "OperatingStatus DisjointWith SoftwareIdentity"^^xsd:string ;
   ontodebug:type "true"^^xsd:boolean
 ] .

[ ontodebug:axiom "Product SubClassOf ManagedSystemElement"^^xsd:string ;
   ontodebug:type "false"^^xsd:boolean
 ] .

[ ontodebug:axiom "Unknown Type Classifications"^^xsd:string ;
   ontodebug:type "true"^^xsd:boolean
 ] .

[ ontodebug:axiom "Classifications DisjointWith OperatingStatus"^^xsd:string ;
   ontodebug:type "true"^^xsd:boolean
 ] .

[ ontodebug:axiom "hasName Domain ManagedSystemElement"^^xsd:string ;
   ontodebug:type "true"^^xsd:boolean
 ] .

[ ontodebug:axiom "Manufacturer Domain ManagedElement"^^xsd:string ;
   ontodebug:type "true"^^xsd:boolean
 ] .

[ ontodebug:axiom "SPDX SubClassOf ManagedSystemElement"^^xsd:string ;
   ontodebug:type "true"^^xsd:boolean
 ] .

[ ontodebug:axiom "Classifications SubClassOf Product"^^xsd:string ;
   ontodebug:type "false"^^xsd:boolean
 ] .

[ ontodebug:axiom "hasName Domain ManagedSystemElement"^^xsd:string ;
   ontodebug:type "true"^^xsd:boolean
 ] .

[ ontodebug:axiom "ManagedSystemElement DisjointWith Product"^^xsd:string ;
   ontodebug:type "true"^^xsd:boolean
 ] .

[ ontodebug:axiom "WarrantyDuration Domain SoftwareIdentity"^^xsd:string ;
   ontodebug:type "false"^^xsd:boolean
 ] .

[ ontodebug:axiom "FRU SubClassOf ManagedSystemElement"^^xsd:string ;
   ontodebug:type "false"^^xsd:boolean
 ] .

[ ontodebug:axiom "Manufacturer Domain ManagedElement"^^xsd:string ;
   ontodebug:type "true"^^xsd:boolean
 ] .

[ ontodebug:axiom "hasName Domain ManagedSystemElement"^^xsd:string ;
   ontodebug:type "true"^^xsd:boolean
 ] .

[ ontodebug:axiom "hasProduct Range PhysicalElement"^^xsd:string ;
   ontodebug:type "true"^^xsd:boolean
 ] .

[ ontodebug:axiom "SPDX EquivalentTo SWID"^^xsd:string ;
   ontodebug:type "false"^^xsd:boolean
 ] .

[ ontodebug:axiom "Product DisjointWith SoftwareIdentity"^^xsd:string ;
   ontodebug:type "true"^^xsd:boolean
 ] .

[ ontodebug:axiom "hasLocation Range SoftwareIdentity"^^xsd:string ;
   ontodebug:type "false"^^xsd:boolean
 ] .

[ ontodebug:axiom "Product DisjointWith SoftwareIdentity"^^xsd:string ;
   ontodebug:type "true"^^xsd:boolean
 ] .

[ ontodebug:axiom "ManagedSystemElement DisjointWith Product"^^xsd:string ;
   ontodebug:type "true"^^xsd:boolean
 ] .

[ ontodebug:axiom "hasName Domain ManagedSystemElement"^^xsd:string ;
   ontodebug:type "true"^^xsd:boolean
 ] .

[ ontodebug:axiom "OperatingStatus DisjointWith SoftwareIdentity"^^xsd:string ;
   ontodebug:type "true"^^xsd:boolean
 ] .

[ ontodebug:axiom "WarrantyDuration Domain SPDX"^^xsd:string ;
   ontodebug:type "false"^^xsd:boolean
 ] .

[ ontodebug:axiom "Name Domain PhysicalElement"^^xsd:string ;
   ontodebug:type "true"^^xsd:boolean
 ] .

[ ontodebug:axiom "Manufacturer Domain SoftwareIdentity"^^xsd:string ;
   ontodebug:type "false"^^xsd:boolean
 ] .

[ ontodebug:axiom "FRU SubClassOf ManagedSystemElement"^^xsd:string ;
   ontodebug:type "false"^^xsd:boolean
 ] .

[ ontodebug:axiom "Manufacturer Domain ManagedElement"^^xsd:string ;
   ontodebug:type "true"^^xsd:boolean
 ] .

[ ontodebug:axiom "Classifications DisjointWith OperatingStatus"^^xsd:string ;
   ontodebug:type "true"^^xsd:boolean
 ] .

[ ontodebug:axiom "Family Domain FRU"^^xsd:string ;
   ontodebug:type "false"^^xsd:boolean
 ] .

[ ontodebug:axiom "Classifications SubClassOf Product"^^xsd:string ;
   ontodebug:type "false"^^xsd:boolean
 ] .

[ ontodebug:axiom "SerialNumber Domain PhysicalElement"^^xsd:string ;
   ontodebug:type "true"^^xsd:boolean
 ] .

[ ontodebug:axiom "hasFRU Range FRU"^^xsd:string ;
   ontodebug:type "true"^^xsd:boolean
 ] .

[ ontodebug:axiom "WarrantyDuration Domain SoftwareIdentity"^^xsd:string ;
   ontodebug:type "false"^^xsd:boolean
 ] .

[ ontodebug:axiom "hasLocation Range SoftwareIdentity"^^xsd:string ;
   ontodebug:type "false"^^xsd:boolean
 ] .

[ ontodebug:axiom "hasProduct Range ManagedElement"^^xsd:string ;
   ontodebug:type "true"^^xsd:boolean
 ] .

[ ontodebug:axiom "SPDX SubClassOf ManagedSystemElement"^^xsd:string ;
   ontodebug:type "true"^^xsd:boolean
 ] .

[ ontodebug:axiom "OperatingStatus Domain PhysicalElement"^^xsd:string ;
   ontodebug:type "true"^^xsd:boolean
 ] .

[ ontodebug:axiom "CISCO_CATALYST_3750 Caption \"Cisco Catalyst 3750\"^^string"^^xsd:string ;
   ontodebug:type "true"^^xsd:boolean
 ] .

[ ontodebug:axiom "Unknown Type Classifications"^^xsd:string ;
   ontodebug:type "true"^^xsd:boolean
 ] .

[ ontodebug:axiom "hasName Domain ManagedElement"^^xsd:string ;
   ontodebug:type "true"^^xsd:boolean
 ] .

[ ontodebug:axiom "SoftwareCreator Domain PhysicalElement"^^xsd:string ;
   ontodebug:type "false"^^xsd:boolean
 ] .

[ ontodebug:axiom "hasFRU Domain Product"^^xsd:string ;
   ontodebug:type "false"^^xsd:boolean
 ] .

[ ontodebug:axiom "Family Domain FRU"^^xsd:string ;
   ontodebug:type "false"^^xsd:boolean
 ] .

[ ontodebug:axiom "Location SubClassOf ManagedSystemElement"^^xsd:string ;
   ontodebug:type "false"^^xsd:boolean
 ] .

[ ontodebug:axiom "hasFRU Domain Product"^^xsd:string ;
   ontodebug:type "false"^^xsd:boolean
 ] .

[ ontodebug:axiom "hasFRU Range FRU"^^xsd:string ;
   ontodebug:type "true"^^xsd:boolean
 ] .

[ ontodebug:axiom "Manufacturer Domain SoftwareIdentity"^^xsd:string ;
   ontodebug:type "false"^^xsd:boolean
 ] .

[ ontodebug:axiom "Caption Domain FRU"^^xsd:string ;
   ontodebug:type "true"^^xsd:boolean
 ] .

[ ontodebug:axiom "hasName Domain ManagedSystemElement"^^xsd:string ;
   ontodebug:type "true"^^xsd:boolean
 ] .

[ ontodebug:axiom "hasProduct Range SPDX"^^xsd:string ;
   ontodebug:type "true"^^xsd:boolean
 ] .

[ ontodebug:axiom "Product SubClassOf ManagedSystemElement"^^xsd:string ;
   ontodebug:type "false"^^xsd:boolean
 ] .

###  Generated by the OWL API (version 4.5.9.2019-02-01T07:24:44Z) https://github.com/owlcs/owlapi
